proof/invariant-abstract/RISCV64/ArchCSpacePre_AI.thy
@@ -201,15 +201,9 @@ lemma valid_arch_mdb_weak_derived_update:
             (caps_of_state s(dest \<mapsto> cap, src \<mapsto> NullCap))"
   by (auto simp: valid_arch_mdb_def)
 
-lemma valid_arch_mdb_tcb_cnode_update:
-  "valid_arch_mdb (is_original_cap s) (caps_of_state s) \<Longrightarrow>
-           valid_arch_mdb ((is_original_cap s) ((t, tcb_cnode_index 2) := True))
-              (caps_of_state s((t, tcb_cnode_index 2) \<mapsto> ReplyCap t True canReplyGrant))"
-  by (clarsimp simp: valid_arch_mdb_def)
-
 lemmas valid_arch_mdb_updates = valid_arch_mdb_free_index_update valid_arch_mdb_not_arch_cap_update
                                 valid_arch_mdb_derived_cap_update valid_arch_mdb_free_index_update'
-                                valid_arch_mdb_weak_derived_update valid_arch_mdb_tcb_cnode_update
+                                valid_arch_mdb_weak_derived_update
 
 lemma safe_parent_for_arch_not_arch':
   "\<not>is_arch_cap cap \<Longrightarrow> \<not>safe_parent_for_arch c cap"
