proof/invariant-abstract/RISCV64/ArchDetSchedSchedule_AI.thy
@@ -12,309 +12,418 @@ context Arch begin global_naming RISCV64
 
 named_theorems DetSchedSchedule_AI_assms
 
-crunch  prepare_thread_delete_idle_thread[wp, DetSchedSchedule_AI_assms]:
-  prepare_thread_delete "\<lambda>(s:: det_ext state). P (idle_thread s)"
+(* trivial functions *)
+crunches arch_post_cap_deletion,
+         prepare_thread_delete,
+         arch_post_modify_registers,
+         arch_get_sanitise_register_info,
+         arch_activate_idle_thread, handle_arch_fault_reply
+  for inv[wp]: P
 
-crunch valid_etcbs [wp, DetSchedSchedule_AI_assms]:
-  arch_switch_to_idle_thread, arch_switch_to_thread, arch_get_sanitise_register_info, arch_post_modify_registers valid_etcbs
-  (simp: crunch_simps)
+(* effects on last_machine_time *)
+crunches setIRQTrigger, maskInterrupt, storeWord, freeMemory, ackDeadlineIRQ, clearMemory,
+         ackInterrupt, hwASIDFlush, read_sbadaddr, setVSpaceRoot, sfence, plic_complete_claim
+  for machine_times[wp]: "\<lambda>s. P (last_machine_time s) (time_state s)"
 
-crunch valid_queues [wp, DetSchedSchedule_AI_assms]:
-  switch_to_idle_thread, switch_to_thread, set_vm_root, arch_get_sanitise_register_info, arch_post_modify_registers valid_queues
-  (simp: crunch_simps ignore: set_tcb_queue tcb_sched_action)
+lemma misc_dmo_valid_sched_pred_strong[wp]:
+  "do_machine_op ackDeadlineIRQ  \<lbrace>valid_sched_pred_strong Q\<rbrace>"
+  "do_machine_op read_sbadaddr  \<lbrace>valid_sched_pred_strong Q\<rbrace>"
+  "do_machine_op sfence \<lbrace>valid_sched_pred_strong Q\<rbrace>"
+  "\<And>a. do_machine_op (plic_complete_claim a) \<lbrace>valid_sched_pred_strong Q\<rbrace>"
+  "\<And>a. do_machine_op (hwASIDFlush a)  \<lbrace>valid_sched_pred_strong Q\<rbrace>"
+  "\<And>a. do_machine_op (ackInterrupt a) \<lbrace>valid_sched_pred_strong Q\<rbrace>"
+  "\<And>a b. do_machine_op (setVSpaceRoot a b) \<lbrace>valid_sched_pred_strong Q\<rbrace>"
+  "\<And>a b. do_machine_op (clearMemory a b) \<lbrace>valid_sched_pred_strong Q\<rbrace>"
+  "\<And>a b. do_machine_op (setIRQTrigger a b) \<lbrace>valid_sched_pred_strong Q\<rbrace>"
+  "\<And>a b. do_machine_op (maskInterrupt a b) \<lbrace>valid_sched_pred_strong Q\<rbrace>"
+  "\<And>a b. do_machine_op (freeMemory a b) \<lbrace>valid_sched_pred_strong Q\<rbrace>"
+  "\<And>a b. do_machine_op (storeWord a b) \<lbrace>valid_sched_pred_strong Q\<rbrace>"
+  by (wpsimp wp: dmo_valid_sched_pred )+
 
-crunch weak_valid_sched_action [wp, DetSchedSchedule_AI_assms]:
-  switch_to_idle_thread, switch_to_thread, set_vm_root, arch_get_sanitise_register_info, arch_post_modify_registers "weak_valid_sched_action"
-  (simp: crunch_simps)
+crunches arch_switch_to_thread,
+         arch_switch_to_idle_thread,
+         arch_finalise_cap,
+         arch_invoke_irq_control,
+         handle_vm_fault
+  for valid_sched_pred_strong[wp, DetSchedSchedule_AI_assms]: "valid_sched_pred_strong P"
+  (wp: dmo_valid_sched_pred crunch_wps simp: crunch_simps)
 
-crunch ct_not_in_q[wp]: set_vm_root "ct_not_in_q"
-  (wp: crunch_wps simp: crunch_simps)
+crunches
+  perform_page_table_invocation,
+  perform_page_invocation, perform_asid_pool_invocation
+  for valid_sched_misc[wp]: "valid_sched_pred_strong P"
+  (wp: dmo_valid_sched_pred crunch_wps simp: crunch_simps detype_def ignore: do_machine_op)
 
-crunch ct_not_in_q'[wp]: set_vm_root "\<lambda>s. ct_not_in_q_2 (ready_queues s) (scheduler_action s) t"
-  (wp: crunch_wps simp: crunch_simps)
 
-lemma switch_to_idle_thread_ct_not_in_q [wp, DetSchedSchedule_AI_assms]:
-  "\<lbrace>valid_queues and valid_idle\<rbrace> switch_to_idle_thread \<lbrace>\<lambda>_. ct_not_in_q\<rbrace>"
-  apply (simp add: switch_to_idle_thread_def)
-  apply wp
-   apply (simp add: arch_switch_to_idle_thread_def)
-   apply wp+
-  apply (fastforce simp: valid_queues_def ct_not_in_q_def not_queued_def
-                         valid_idle_def pred_tcb_at_def obj_at_def)
-  done
+crunches arch_perform_invocation
+  for valid_sched_misc[wp, DetSchedSchedule_AI_assms]:
+        "\<lambda>s. P (consumed_time s) (cur_time s) (cur_domain s) (cur_thread s)
+               (cur_sc s) (idle_thread s) (ready_queues s) (release_queue s)
+               (scheduler_action s) (last_machine_time_of s) (time_state_of s)"
+  (wp: dmo_valid_sched_pred crunch_wps simp: crunch_simps detype_def ignore: do_machine_op)
 
-crunch valid_sched_action'[wp]: set_vm_root "\<lambda>s. valid_sched_action_2 (scheduler_action s)
-                                                 (ekheap s) (kheap s) thread (cur_domain s)"
-  (wp: crunch_wps simp: crunch_simps)
-
-lemma switch_to_idle_thread_valid_sched_action [wp, DetSchedSchedule_AI_assms]:
-  "\<lbrace>valid_sched_action and valid_idle\<rbrace>
-     switch_to_idle_thread
-   \<lbrace>\<lambda>_. valid_sched_action\<rbrace>"
-  apply (simp add: switch_to_idle_thread_def)
-  apply wp
-   apply (simp add: arch_switch_to_idle_thread_def do_machine_op_def split_def)
-   apply wp+
-  apply (clarsimp simp: valid_sched_action_def valid_idle_def is_activatable_def
-                        pred_tcb_at_def obj_at_def)
-  done
-
-crunch ct_in_cur_domain'[wp]: set_vm_root "\<lambda>s. ct_in_cur_domain_2 t (idle_thread s)
-                                                   (scheduler_action s) (cur_domain s) (ekheap s)"
-  (wp: crunch_wps simp: crunch_simps)
-
-lemma switch_to_idle_thread_ct_in_cur_domain [wp, DetSchedSchedule_AI_assms]:
+lemma switch_to_idle_thread_ct_in_cur_domain [wp]:
   "\<lbrace>\<top>\<rbrace> switch_to_idle_thread \<lbrace>\<lambda>_. ct_in_cur_domain\<rbrace>"
   by (simp add: switch_to_idle_thread_def arch_switch_to_idle_thread_def do_machine_op_def
                 split_def
       | wp
       | simp add: ct_in_cur_domain_def)+
 
-crunch ct_not_in_q [wp, DetSchedSchedule_AI_assms]: arch_switch_to_thread, arch_get_sanitise_register_info, arch_post_modify_registers ct_not_in_q
-  (simp: crunch_simps wp: crunch_wps)
-
-crunch is_activatable [wp, DetSchedSchedule_AI_assms]: arch_switch_to_thread, arch_get_sanitise_register_info, arch_post_modify_registers "is_activatable t"
-  (simp: crunch_simps)
-
-crunch valid_sched_action [wp, DetSchedSchedule_AI_assms]: arch_switch_to_thread, arch_get_sanitise_register_info, arch_post_modify_registers valid_sched_action
-  (simp: crunch_simps)
-
-crunch valid_sched [wp, DetSchedSchedule_AI_assms]: arch_switch_to_thread, arch_get_sanitise_register_info, arch_post_modify_registers valid_sched
-  (simp: crunch_simps)
-
 crunch exst[wp]: set_vm_root "\<lambda>s. P (exst s)"
   (wp: crunch_wps hoare_whenE_wp simp: crunch_simps)
 
-crunch ct_in_cur_domain_2 [wp, DetSchedSchedule_AI_assms]: arch_switch_to_thread
-  "\<lambda>s. ct_in_cur_domain_2 thread (idle_thread s) (scheduler_action s) (cur_domain s) (ekheap s)"
-  (simp: crunch_simps wp: assert_inv)
+crunch etcb_at[wp]: switch_to_thread "etcb_at P t"
+  (wp: hoare_drop_imp)
 
-crunch valid_blocked[wp]: set_vm_root valid_blocked
-  (simp: crunch_simps)
-
-crunch ct_in_q[wp]: set_vm_root ct_in_q
-  (simp: crunch_simps)
-
-crunch etcb_at [wp, DetSchedSchedule_AI_assms]: switch_to_thread "etcb_at P t"
-
-crunch valid_idle [wp, DetSchedSchedule_AI_assms]:
+crunch valid_idle [wp]:
   arch_switch_to_idle_thread "valid_idle"
   (wp: crunch_wps simp: crunch_simps)
-
-crunch etcb_at [wp, DetSchedSchedule_AI_assms]: arch_switch_to_idle_thread "etcb_at P t"
-
-crunch scheduler_action [wp, DetSchedSchedule_AI_assms]:
-  arch_switch_to_idle_thread, next_domain "\<lambda>s. P (scheduler_action s)"
-  (simp: Let_def)
 
 lemma set_vm_root_valid_blocked_ct_in_q [wp]:
   "\<lbrace>valid_blocked and ct_in_q\<rbrace> set_vm_root p \<lbrace>\<lambda>_. valid_blocked and ct_in_q\<rbrace>"
   by (wp | wpc | auto)+
 
+lemma arch_switch_to_thread_valid_blocked [wp]:
+  "\<lbrace>valid_blocked and ct_in_q\<rbrace> arch_switch_to_thread thread \<lbrace>\<lambda>_. valid_blocked and ct_in_q::det_state \<Rightarrow> _\<rbrace>"
+  unfolding arch_switch_to_thread_def by wpsimp
 
-lemma as_user_ct_in_q[wp]:
-  "as_user tp S \<lbrace>ct_in_q\<rbrace>"
-  apply (wpsimp simp: as_user_def set_object_def get_object_def)
-  apply (clarsimp simp: ct_in_q_def st_tcb_at_def obj_at_def dest!: get_tcb_SomeD)
-  done
-
-lemma arch_switch_to_thread_valid_blocked [wp, DetSchedSchedule_AI_assms]:
-  "\<lbrace>valid_blocked and ct_in_q\<rbrace> arch_switch_to_thread thread \<lbrace>\<lambda>_. valid_blocked and ct_in_q\<rbrace>"
-  by (wpsimp simp: arch_switch_to_thread_def)
-
-lemma switch_to_idle_thread_ct_not_queued [wp, DetSchedSchedule_AI_assms]:
-  "\<lbrace>valid_queues and valid_etcbs and valid_idle\<rbrace>
+lemma switch_to_idle_thread_ct_not_queued [wp]:
+  "\<lbrace>valid_ready_qs and valid_idle\<rbrace>
      switch_to_idle_thread
    \<lbrace>\<lambda>rv s. not_queued (cur_thread s) s\<rbrace>"
   apply (simp add: switch_to_idle_thread_def arch_switch_to_idle_thread_def
                    tcb_sched_action_def | wp)+
-  apply (fastforce simp: valid_sched_2_def valid_queues_2_def valid_idle_def
-                         pred_tcb_at_def obj_at_def not_queued_def)
+  apply (clarsimp simp: valid_sched_def valid_ready_qs_def valid_idle_def
+                        pred_tcb_at_def obj_at_def not_queued_def pred_map_simps vs_all_heap_simps
+         , fastforce)
   done
 
-crunch valid_blocked_2[wp]: set_vm_root "\<lambda>s.
-           valid_blocked_2 (ready_queues s) (kheap s)
-            (scheduler_action s) thread"
-  (wp: crunch_wps simp: crunch_simps)
-
-lemma switch_to_idle_thread_valid_blocked [wp, DetSchedSchedule_AI_assms]:
-  "\<lbrace>valid_blocked and ct_in_q\<rbrace> switch_to_idle_thread \<lbrace>\<lambda>rv. valid_blocked\<rbrace>"
-  apply (simp add: switch_to_idle_thread_def arch_switch_to_idle_thread_def do_machine_op_def | wp | wpc)+
-  apply clarsimp
-  apply (drule(1) ct_in_q_valid_blocked_ct_upd)
-  apply simp
-  done
-
-crunch exst [wp, DetSchedSchedule_AI_assms]: arch_switch_to_thread "\<lambda>s. P (exst s :: det_ext)"
-
-crunch cur_thread[wp]: arch_switch_to_idle_thread "\<lambda>s. P (cur_thread s)"
+crunch exst [wp]: arch_switch_to_thread "\<lambda>s. P (exst s :: det_ext)"
 
 lemma astit_st_tcb_at[wp]:
   "\<lbrace>st_tcb_at P t\<rbrace> arch_switch_to_idle_thread \<lbrace>\<lambda>rv. st_tcb_at P t\<rbrace>"
   apply (simp add: arch_switch_to_idle_thread_def)
   by (wpsimp)
 
-lemma stit_activatable' [DetSchedSchedule_AI_assms]:
+lemma stit_activatable':
   "\<lbrace>valid_idle\<rbrace> switch_to_idle_thread \<lbrace>\<lambda>rv . ct_in_state activatable\<rbrace>"
   apply (simp add: switch_to_idle_thread_def ct_in_state_def do_machine_op_def split_def)
   apply wpsimp
   apply (clarsimp simp: valid_idle_def ct_in_state_def pred_tcb_at_def obj_at_def)
   done
 
-lemma switch_to_idle_thread_cur_thread_idle_thread [wp, DetSchedSchedule_AI_assms]:
+lemma switch_to_idle_thread_cur_thread_idle_thread [wp]:
   "\<lbrace>\<top>\<rbrace> switch_to_idle_thread \<lbrace>\<lambda>_ s. cur_thread s = idle_thread s\<rbrace>"
   by (wp | simp add:switch_to_idle_thread_def arch_switch_to_idle_thread_def)+
 
-lemma set_pt_valid_etcbs[wp]:
-  "\<lbrace>valid_etcbs\<rbrace> set_pt ptr pt \<lbrace>\<lambda>rv. valid_etcbs\<rbrace>"
-  by (wp hoare_drop_imps valid_etcbs_lift | simp add: set_pt_def)+
+lemma set_thread_state_cur_thread_valid_blocked:
+  "\<lbrace>valid_blocked and (\<lambda>s. ref = cur_thread s)\<rbrace> set_thread_state ref ts
+  \<lbrace>\<lambda>_. valid_blocked :: det_state \<Rightarrow> _\<rbrace>"
+  by (wp set_thread_state_valid_blocked_const | wps)+ clarsimp
 
-lemma set_asid_pool_valid_etcbs[wp]:
-  "\<lbrace>valid_etcbs\<rbrace> set_asid_pool ptr pool \<lbrace>\<lambda>rv. valid_etcbs\<rbrace>"
-  by (wp hoare_drop_imps valid_etcbs_lift | simp add: set_asid_pool_def)+
+(* FIXME: move out of arch *)
+lemma set_thread_state_cur_thread_runnable_valid_sched:
+  "\<lbrace>valid_sched and (\<lambda>s. ref = cur_thread s) and K (runnable ts)\<rbrace>
+   set_thread_state ref ts
+   \<lbrace>\<lambda>_. valid_sched :: det_state \<Rightarrow> _\<rbrace>"
+  apply (wpsimp wp: set_thread_state_valid_sched)
+  by (clarsimp simp: valid_sched_def runnable_eq, fastforce)
 
-lemma set_pt_valid_sched[wp]:
-  "\<lbrace>valid_sched\<rbrace> set_pt ptr pt \<lbrace>\<lambda>rv. valid_sched\<rbrace>"
-  by (wp hoare_drop_imps valid_sched_lift | simp add: set_pt_def)+
-
-lemma set_asid_pool_valid_sched[wp]:
-  "\<lbrace>valid_sched\<rbrace> set_asid_pool ptr pool \<lbrace>\<lambda>rv. valid_sched\<rbrace>"
-  by (wp hoare_drop_imps valid_sched_lift | simp add: set_asid_pool_def)+
-
-crunch ct_not_in_q [wp, DetSchedSchedule_AI_assms]:
-  arch_finalise_cap, prepare_thread_delete ct_not_in_q
-  (wp: crunch_wps hoare_drop_imps hoare_unless_wp select_inv mapM_wp
-       subset_refl if_fun_split simp: crunch_simps ignore: tcb_sched_action)
-
-crunch valid_etcbs [wp, DetSchedSchedule_AI_assms]:
-  arch_finalise_cap, prepare_thread_delete valid_etcbs
-  (wp: hoare_drop_imps hoare_unless_wp select_inv mapM_x_wp mapM_wp subset_refl
-       if_fun_split simp: crunch_simps ignore: set_object thread_set)
-
-crunch simple_sched_action [wp, DetSchedSchedule_AI_assms]:
-  arch_finalise_cap, prepare_thread_delete simple_sched_action
-  (wp: hoare_drop_imps mapM_x_wp mapM_wp select_wp subset_refl
-   simp: unless_def if_fun_split)
-
-crunch valid_sched [wp, DetSchedSchedule_AI_assms]:
-  arch_finalise_cap, prepare_thread_delete, arch_invoke_irq_handler, arch_mask_irq_signal
-  "valid_sched"
-  (ignore: set_object wp: crunch_wps subset_refl simp: if_fun_split)
-
-lemma activate_thread_valid_sched [DetSchedSchedule_AI_assms]:
-  "\<lbrace>valid_sched\<rbrace> activate_thread \<lbrace>\<lambda>_. valid_sched\<rbrace>"
-  apply (simp add: activate_thread_def)
-  apply (wp set_thread_state_runnable_valid_sched gts_wp | wpc | simp add: arch_activate_idle_thread_def)+
-  apply (force elim: st_tcb_weakenE)
-  done
-
-crunch valid_sched[wp]:
-  perform_page_invocation, perform_page_table_invocation, perform_asid_pool_invocation
-  valid_sched
-  (wp: mapM_x_wp' mapM_wp' crunch_wps)
+lemma activate_thread_valid_sched:
+  "\<lbrace>valid_sched\<rbrace>
+   activate_thread
+   \<lbrace>\<lambda>_. valid_sched :: det_state \<Rightarrow> _\<rbrace>"
+  unfolding activate_thread_def
+  by (wpsimp wp: set_thread_state_cur_thread_runnable_valid_sched gts_wp hoare_vcg_all_lift
+                 get_tcb_obj_ref_wp hoare_drop_imps)
 
 lemma arch_perform_invocation_valid_sched [wp, DetSchedSchedule_AI_assms]:
-  "\<lbrace>invs and valid_sched and ct_active and valid_arch_inv a\<rbrace>
+  "\<lbrace>invs and valid_sched and ct_active and (\<lambda>s. scheduler_action s = resume_cur_thread) and
+    valid_arch_inv a\<rbrace>
      arch_perform_invocation a
-   \<lbrace>\<lambda>_.valid_sched\<rbrace>"
+   \<lbrace>\<lambda>_. valid_sched\<rbrace>"
   apply (cases a, simp_all add: arch_perform_invocation_def)
-     apply (wp perform_asid_control_invocation_valid_sched | wpc |
-            simp add: valid_arch_inv_def invs_valid_idle)+
+      apply (wpsimp simp: valid_arch_inv_def invs_valid_idle
+                      wp: perform_asid_control_invocation_valid_sched)+
   done
 
-crunch valid_sched [wp, DetSchedSchedule_AI_assms]:
-  handle_arch_fault_reply, handle_vm_fault valid_sched
-  (simp: crunch_simps)
-
-crunch not_queued [wp, DetSchedSchedule_AI_assms]:
-  handle_vm_fault, handle_arch_fault_reply "not_queued t"
-  (simp: crunch_simps)
-
-crunch sched_act_not [wp, DetSchedSchedule_AI_assms]:
-  handle_arch_fault_reply, handle_vm_fault "scheduler_act_not t"
-  (simp: crunch_simps)
-
-lemma hvmf_st_tcb_at [wp, DetSchedSchedule_AI_assms]:
-  "\<lbrace>st_tcb_at P t' \<rbrace> handle_vm_fault t w \<lbrace>\<lambda>rv. st_tcb_at P t' \<rbrace>"
-  unfolding handle_vm_fault_def by (cases w; wpsimp)
-
-lemma handle_vm_fault_st_tcb_cur_thread [wp, DetSchedSchedule_AI_assms]:
+lemma handle_vm_fault_st_tcb_cur_thread [wp]:
   "\<lbrace> \<lambda>s. st_tcb_at P (cur_thread s) s \<rbrace> handle_vm_fault t f \<lbrace>\<lambda>_ s. st_tcb_at P (cur_thread s) s \<rbrace>"
-  unfolding handle_vm_fault_def
   apply (fold ct_in_state_def)
-  apply (rule ct_in_state_thread_state_lift; cases f; wpsimp)
+  apply (rule ct_in_state_thread_state_lift)
+   apply (cases f)
+    apply (wp|simp)+
   done
 
-crunch valid_sched [wp, DetSchedSchedule_AI_assms]: arch_invoke_irq_control "valid_sched"
+crunches arch_switch_to_thread, arch_switch_to_idle_thread
+  for valid_list [wp]: "valid_list"
 
-crunch valid_list [wp, DetSchedSchedule_AI_assms]:
-  arch_activate_idle_thread, arch_switch_to_thread, arch_switch_to_idle_thread "valid_list"
+crunch cur_tcb [wp]: handle_arch_fault_reply, handle_vm_fault, arch_post_modify_registers cur_tcb
 
-crunch cur_tcb [wp, DetSchedSchedule_AI_assms]:
-  handle_arch_fault_reply, handle_vm_fault, arch_get_sanitise_register_info, arch_post_modify_registers
-  cur_tcb
+(* FIXME: move out of arch *)
+lemma valid_idle_thread_state_contradiction:
+  "valid_idle s \<Longrightarrow> pred_map P (tcb_sts_of s) (idle_thread s) \<Longrightarrow> \<not> P (IdleThreadState) \<Longrightarrow> False"
+  unfolding valid_idle_def
+  by (clarsimp simp: tcb_at_kh_simps vs_all_heap_simps pred_tcb_at_def obj_at_def)
+
+lemma switch_to_idle_thread_ct_not_in_release_q[wp]:
+    "\<lbrace>valid_release_q and valid_idle\<rbrace>
+      switch_to_idle_thread
+     \<lbrace>\<lambda>rv s::det_state. ct_not_in_release_q s\<rbrace>"
+  apply (clarsimp simp: switch_to_idle_thread_def)
+  apply wpsimp
+  by (fastforce simp: valid_release_q_def not_in_release_q_def in_queue_2_def dest!: valid_idle_thread_state_contradiction)
+
+crunches arch_switch_to_thread, arch_switch_to_idle_thread
+  for sc_at_period[wp]: "sc_at_period P p::det_state \<Rightarrow> _"
   (simp: crunch_simps)
 
-crunch not_cur_thread [wp, DetSchedSchedule_AI_assms]: arch_get_sanitise_register_info, arch_post_modify_registers "not_cur_thread t'"
-crunch ready_queues   [wp, DetSchedSchedule_AI_assms]: arch_get_sanitise_register_info, arch_post_modify_registers "\<lambda>s. P (ready_queues s)"
-crunch scheduler_action [wp, DetSchedSchedule_AI_assms]: arch_get_sanitise_register_info, arch_post_modify_registers "\<lambda>s. P (scheduler_action s)"
+lemma machine_state_detype[simp]:
+  "machine_state (detype S s) = machine_state s"
+  by (clarsimp simp: valid_machine_time_def detype_def)
 
-lemma make_arch_fault_msg_inv:
-  "make_arch_fault_msg f t \<lbrace>P\<rbrace>"
-  by (cases f) wpsimp
+crunches handle_hypervisor_fault, handle_reserved_irq
+  for valid_machine_time: valid_machine_time
 
-declare make_arch_fault_msg_inv[DetSchedSchedule_AI_assms]
+lemma valid_machine_time_getCurrentTime:
+  "\<And>s x s'. valid_machine_time s \<Longrightarrow> (x, s') \<in> fst (getCurrentTime (machine_state s)) \<Longrightarrow>
+            valid_machine_time_2 x (last_machine_time s')"
+  apply (clarsimp simp: valid_machine_time_def getCurrentTime_def in_monad)
+  apply (rule word_of_nat_le)
+  apply (rule Lattices.linorder_class.min.coboundedI1)
+  apply (subst unat_minus_one)
+   using kernelWCET_ticks_pos2 apply fastforce
+  apply (subst unat_minus')
+   using kernelWCET_ticks_pos2 apply fastforce
+  apply clarsimp
+  done
 
-lemma arch_post_modify_registers_not_idle_thread[DetSchedSchedule_AI_assms]:
-  "\<lbrace>\<lambda>s::det_ext state. t \<noteq> idle_thread s\<rbrace> arch_post_modify_registers c t \<lbrace>\<lambda>_ s. t \<noteq> idle_thread s\<rbrace>"
-  by (wpsimp simp: arch_post_modify_registers_def)
+lemma dmo_getCurrentTime_vmt_sp[wp]:
+  "\<lbrace>valid_machine_time\<rbrace>
+   do_machine_op getCurrentTime
+   \<lbrace>\<lambda>rv s. (cur_time s \<le> rv) \<and> (rv \<le> - kernelWCET_ticks - 1)\<rbrace>"
+  apply (wpsimp simp: do_machine_op_def)
+  apply (clarsimp simp: valid_machine_time_def getCurrentTime_def in_monad)
+  apply (intro conjI)
+   apply (clarsimp simp: min_def, intro conjI impI)
+  subgoal
+    apply (rule_tac order.trans, assumption)
+    apply (rule_tac order.trans, assumption)
+    apply (rule preorder_class.eq_refl)
+    apply (subst group_add_class.diff_conv_add_uminus)
+    apply (subst minus_one_norm_num)
+    apply clarsimp
+    apply (rule word_unat.Rep_inverse'[symmetric])
+    apply (subst unat_sub)
+     apply (rule order.trans[OF word_up_bound])
+     apply (rule preorder_class.eq_refl)
+     apply simp
+    apply simp
+    done
+  subgoal for s
+    apply (subst (asm) linorder_class.not_le)
+    apply (rule_tac order.trans, assumption)
+    apply (rule no_plus_overflow_unat_size2)
+    apply (rule_tac order.trans)
+     apply (rule add_le_mono)
+      apply (rule preorder_class.eq_refl, simp)
+     apply (rule unat_of_nat_closure)
+    apply (rule_tac order.trans)
+     apply (rule order_class.order.strict_implies_order, assumption)
+    apply simp
+    done
+  apply (clarsimp simp: min_def, intro conjI impI)
+  subgoal
+    apply (rule preorder_class.eq_refl)
+    apply (subst group_add_class.diff_conv_add_uminus)
+    apply (subst minus_one_norm_num)
+    apply clarsimp
+    apply (rule word_unat.Rep_inverse')
+    apply (subst unat_sub)
+     apply (rule order.trans[OF word_up_bound])
+     apply (rule preorder_class.eq_refl)
+     apply simp
+    apply simp
+    done
+  subgoal for s
+    apply (subst (asm) linorder_class.not_le)
+    apply (rule_tac b="of_nat (unat (last_machine_time (machine_state s)) +
+      time_oracle (Suc (time_state (machine_state s))))" in order.trans[rotated])
+     apply (rule Word_Lemmas.word_of_nat_le)
+     apply (rule_tac order.trans)
+      apply (rule order.strict_implies_order, assumption)
+     apply (subst group_add_class.diff_conv_add_uminus)
+     apply (subst minus_one_norm_num)
+     apply clarsimp
+     apply (subst unat_sub)
+      apply (rule order.trans[OF word_up_bound])
+      apply (rule preorder_class.eq_refl)
+      apply simp
+     apply simp
+    apply clarsimp
+    done
+  done
 
-crunches arch_post_cap_deletion
-  for valid_sched[wp, DetSchedSchedule_AI_assms]: valid_sched
-  and valid_etcbs[wp, DetSchedSchedule_AI_assms]: valid_etcbs
-  and ct_not_in_q[wp, DetSchedSchedule_AI_assms]: ct_not_in_q
-  and simple_sched_action[wp, DetSchedSchedule_AI_assms]: simple_sched_action
-  and not_cur_thread[wp, DetSchedSchedule_AI_assms]: "not_cur_thread t"
-  and is_etcb_at[wp, DetSchedSchedule_AI_assms]: "is_etcb_at t"
-  and not_queued[wp, DetSchedSchedule_AI_assms]: "not_queued t"
-  and sched_act_not[wp, DetSchedSchedule_AI_assms]: "scheduler_act_not t"
-  and weak_valid_sched_action[wp, DetSchedSchedule_AI_assms]: weak_valid_sched_action
-  and valid_idle[wp, DetSchedSchedule_AI_assms]: valid_idle
+lemma update_time_stamp_valid_machine_time[wp]:
+  "update_time_stamp \<lbrace>valid_machine_time\<rbrace>"
+  unfolding update_time_stamp_def
+  apply (wpsimp simp: do_machine_op_def)
+  apply (fastforce simp: getCurrentTime_def elim: valid_machine_time_getCurrentTime)
+  done
 
-crunch delete_asid_pool[wp]: delete_asid_pool "\<lambda>(s:: det_ext state). P (idle_thread s)"
- (wp: crunch_wps simp: if_apply_def2)
+(* Note: Proving that retype_region preserves bound_sc_tcb_at is much harder *)
+lemma retype_region_not_bound_sc[wp]:
+  "\<lbrace>\<lambda>s. \<not> bound_sc_tcb_at P t s\<rbrace>
+   retype_region ptr' 1 us (ArchObject aobj) dev
+   \<lbrace>\<lambda>rv (s). \<not> bound_sc_tcb_at P t s\<rbrace>"
+  by (wpsimp simp: retype_region_def,
+         clarsimp simp: pred_tcb_at_def sc_at_pred_def obj_at_def default_object_def
+                 split: if_splits)
 
-crunch arch_finalise_cap[wp, DetSchedSchedule_AI_assms]:
-  arch_finalise_cap "\<lambda>(s:: det_ext state). P (idle_thread s)"
-  (wp: crunch_wps simp: if_fun_split)
+crunches arch_perform_invocation
+  for not_bound_sc_tcb_at[wp]: "(\<lambda>s. \<not> bound_sc_tcb_at P t s)"
+  (wp: crunch_wps cur_sc_tcb_only_sym_bound_lift ignore: retype_region delete_objects)
+
+lemma arch_perform_invocation_cur_sc_tcb_only_sym_bound[DetSchedSchedule_AI_assms]:
+  "arch_perform_invocation i \<lbrace>cur_sc_tcb_only_sym_bound\<rbrace>"
+  by (wpsimp wp: cur_sc_tcb_only_sym_bound_lift)
+
+lemma arch_perform_invocation_bound_sc_obj_tcb_at[DetSchedSchedule_AI_assms]:
+  "\<lbrace>\<lambda>s. bound_sc_obj_tcb_at (P (cur_time s)) t s
+        \<and> ex_nonz_cap_to t s \<and> invs s \<and> ct_active s \<and> valid_arch_inv i s
+        \<and> scheduler_action s = resume_cur_thread\<rbrace>
+   arch_perform_invocation i
+   \<lbrace>\<lambda>_ s. bound_sc_obj_tcb_at (P (cur_time s)) t s\<rbrace>"
+  unfolding arch_perform_invocation_def
+  by (cases i; wpsimp simp: valid_arch_inv_def)
+
+lemma arch_finalise_cap_ct_in_state:
+  "arch_finalise_cap c x \<lbrace>ct_in_state P :: det_state \<Rightarrow> _\<rbrace>"
+  apply (case_tac c; case_tac x; simp add: arch_finalise_cap_def)
+  by (wpsimp wp: ct_in_state_thread_state_lift)+
+
+lemma kernel_irq_timer_kernel_IRQ[simp]:
+  "kernel_irq_timer \<notin> non_kernel_IRQs"
+  by (simp add: non_kernel_IRQs_def)
+
+lemma arch_perform_invocationE_E_inv[wp]:
+  "\<lbrace>\<top>\<rbrace> arch_perform_invocation i -, \<lbrace>Q\<rbrace>"
+   unfolding arch_perform_invocation_def by wpsimp
+
+lemma retype_region_cur_sc_more_than_ready [wp]:
+  "retype_region ptr numObjects o_bits type dev \<lbrace>cur_sc_more_than_ready\<rbrace>"
+  apply (rule_tac Q="\<lambda>_ s. \<forall>cons_time csc c_time.
+    cons_time = consumed_time s \<and> csc = cur_sc s \<and> c_time = cur_time s \<longrightarrow>
+    (cons_time \<noteq> 0
+    \<longrightarrow> pred_map active_scrc (sc_refill_cfgs_of s) csc
+    \<longrightarrow> pred_map (refill_ready_no_overflow_sc cons_time c_time) (sc_refill_cfgs_of s) csc
+         \<and> pred_map (refill_sufficient_sc cons_time) (sc_refill_cfgs_of s) csc)" in hoare_strengthen_post)
+   apply (wp hoare_vcg_all_lift)
+    apply (rule hoare_vcg_imp_lift'[rotated])
+     apply (rule hoare_vcg_imp_lift'[rotated])
+      apply (subst imp_conjR)
+      apply (wp retype_region_active_sc_props)
+     apply wpsimp+
+   apply (clarsimp simp: cur_sc_more_than_ready_def)
+  apply (clarsimp simp: cur_sc_more_than_ready_def)
+  done
+
+lemma delete_objects_cur_sc_more_than_ready [wp]:
+  "delete_objects ptr pagebits \<lbrace>cur_sc_more_than_ready\<rbrace>"
+  apply (rule_tac Q="\<lambda>_ s. \<forall>cons_time csc c_time.
+    cons_time = consumed_time s \<and> csc = cur_sc s \<and> c_time = cur_time s \<longrightarrow>
+    (cons_time \<noteq> 0
+    \<longrightarrow> pred_map active_scrc (sc_refill_cfgs_of s) csc
+    \<longrightarrow> pred_map (refill_ready_no_overflow_sc cons_time c_time) (sc_refill_cfgs_of s) csc
+         \<and> pred_map (refill_sufficient_sc cons_time) (sc_refill_cfgs_of s) csc)" in hoare_strengthen_post)
+   apply (wp hoare_vcg_all_lift)
+    apply (rule hoare_vcg_imp_lift'[rotated])
+     apply (rule hoare_vcg_imp_lift'[rotated])
+      apply (subst imp_conjR)
+      apply (wp delete_objects_pred_map_sc_refill_cfgs_of)
+     apply wpsimp+
+   apply (clarsimp simp: cur_sc_more_than_ready_def)
+  apply (clarsimp simp: cur_sc_more_than_ready_def)
+  done
+
+lemma perform_asid_control_invocation_cur_sc_more_than_ready [wp]:
+  "perform_asid_control_invocation iv \<lbrace>cur_sc_more_than_ready\<rbrace>"
+  unfolding perform_asid_control_invocation_def
+  by (wpsimp wp: hoare_drop_imp)
+
+lemma arch_perform_invocation_cur_sc_more_than_ready [wp, DetSchedSchedule_AI_assms]:
+  "arch_perform_invocation iv \<lbrace>cur_sc_more_than_ready\<rbrace>"
+  unfolding arch_perform_invocation_def
+  by (cases iv; wpsimp)
+
+lemma perform_asid_control_invocation_cur_sc_in_release_q_imp_zero_consumed [wp]:
+  "perform_asid_control_invocation iv \<lbrace>cur_sc_in_release_q_imp_zero_consumed\<rbrace>"
+  unfolding perform_asid_control_invocation_def
+  by (wpsimp wp: hoare_drop_imp)
+
+lemma arch_perform_invocation_cur_sc_in_release_q_imp_zero_consumed [wp, DetSchedSchedule_AI_assms]:
+  "arch_perform_invocation iv \<lbrace>cur_sc_in_release_q_imp_zero_consumed\<rbrace>"
+  unfolding arch_perform_invocation_def
+  by (cases iv; wpsimp wp: hoare_drop_imps)
+
+crunches arch_invoke_irq_handler, arch_mask_irq_signal, handle_reserved_irq
+  for ct_active[wp]: ct_active
+
+lemma arch_invoke_irq_handler_valid_sched_pred_strong[wp]:
+  "arch_invoke_irq_handler i \<lbrace> valid_sched_pred_strong P \<rbrace>"
+  by (cases i; wpsimp)
+
+lemma arch_mask_irq_signal_valid_sched_pred_strong[wp]:
+  "arch_mask_irq_signal i \<lbrace> valid_sched_pred_strong P \<rbrace>"
+  unfolding arch_mask_irq_signal_def by wpsimp
+
+crunches arch_switch_to_thread, arch_switch_to_idle_thread
+for cdt_cdt_list_exst [wp]:  "\<lambda>s. P (cdt s) (cdt_list_internal (exst s))"
+
+crunches make_arch_fault_msg
+  for valid_sched_pred_strong[wp,DetSchedSchedule_AI_assms]: "valid_sched_pred_strong P"
 
 end
 
 global_interpretation DetSchedSchedule_AI?: DetSchedSchedule_AI
-  proof goal_cases
+proof goal_cases
   interpret Arch .
-  case 1 show ?case by (unfold_locales; (fact DetSchedSchedule_AI_assms)?)
-  qed
+  case 1 show ?case by (unfold_locales; (fact DetSchedSchedule_AI_assms)?; wpsimp?)
+qed
+
+global_interpretation DetSchedSchedule_AI_det_ext?: DetSchedSchedule_AI_det_ext
+proof goal_cases
+  interpret Arch .
+  case 1 show ?case by (unfold_locales; (fact DetSchedSchedule_AI_assms)?; wpsimp)
+qed
 
 context Arch begin global_naming RISCV64
 
-lemma handle_hyp_fault_valid_sched[wp]:
-  "\<lbrace>valid_sched and invs and st_tcb_at active t and not_queued t and scheduler_act_not t
-      and (ct_active or ct_idle)\<rbrace>
-    handle_hypervisor_fault t fault \<lbrace>\<lambda>_. valid_sched\<rbrace>"
-  by (cases fault; wpsimp wp: handle_fault_valid_sched simp: valid_fault_def)
+lemma handle_hyp_fault_trivial[wp]:
+  "handle_hypervisor_fault t fault \<lbrace>Q\<rbrace>"
+  by (cases fault; wpsimp)
 
-lemma handle_reserved_irq_valid_sched:
-  "\<lbrace>valid_sched and invs and (\<lambda>s. irq \<in> non_kernel_IRQs \<longrightarrow>  scheduler_act_sane s \<and> ct_not_queued s)\<rbrace>
-  handle_reserved_irq irq \<lbrace>\<lambda>rv. valid_sched\<rbrace>"
-  unfolding handle_reserved_irq_def by (wpsimp simp: non_kernel_IRQs_def)
+lemma handle_reserved_irq_trivial[wp]:
+  "handle_reserved_irq irq \<lbrace>Q\<rbrace>"
+  unfolding handle_reserved_irq_def
+  by (wpsimp)
+
+lemma handle_vm_fault_not_timeout_fault[wp]:
+  "\<lbrace>\<top>\<rbrace> handle_vm_fault thread ft -,\<lbrace>\<lambda>rv s. \<not> is_timeout_fault rv\<rbrace>"
+  unfolding handle_vm_fault_def by (wpsimp simp: is_timeout_fault_def)
 
 end
 
 global_interpretation DetSchedSchedule_AI_handle_hypervisor_fault?: DetSchedSchedule_AI_handle_hypervisor_fault
-  proof goal_cases
+proof goal_cases
   interpret Arch .
-  case 1 show ?case by (unfold_locales; (fact handle_hyp_fault_valid_sched handle_reserved_irq_valid_sched)?)
-  qed
+  case 1 show ?case by (unfold_locales; wpsimp)
+qed
+
+global_interpretation DetSchedSchedule_AI_handle_hypervisor_fault_det_ext?: DetSchedSchedule_AI_handle_hypervisor_fault_det_ext
+proof goal_cases
+  interpret Arch .
+  case 1 show ?case by (unfold_locales; wpsimp)
+qed
 
 end
