proof/invariant-abstract/RISCV64/ArchFinalise_AI.thy
@@ -191,7 +191,6 @@ lemmas [Finalise_AI_asms] = obj_refs_obj_ref_of (* used under name obj_ref_ofI *
 
 lemma (* empty_slot_invs *) [Finalise_AI_asms]:
   "\<lbrace>\<lambda>s. invs s \<and> cte_wp_at (replaceable s sl cap.NullCap) sl s \<and>
-        emptyable sl s \<and>
         (info \<noteq> NullCap \<longrightarrow> post_cap_delete_pre info ((caps_of_state s) (sl \<mapsto> NullCap)))\<rbrace>
      empty_slot sl info
    \<lbrace>\<lambda>rv. invs\<rbrace>"
@@ -225,33 +224,15 @@ lemma (* empty_slot_invs *) [Finalise_AI_asms]:
   apply (rule conjI)
    apply (clarsimp simp: irq_revocable_def)
   apply (rule conjI)
-   apply (clarsimp simp: reply_master_revocable_def)
   apply (thin_tac "info \<noteq> NullCap \<longrightarrow> P info" for P)
-  apply (rule conjI)
    apply (clarsimp simp: valid_machine_state_def)
   apply (rule conjI)
    apply (clarsimp simp:descendants_inc_def mdb_empty_abs.descendants)
   apply (rule conjI)
-   apply (clarsimp simp: reply_mdb_def)
-   apply (rule conjI)
-    apply (unfold reply_caps_mdb_def)[1]
-    apply (rule allEI, assumption)
-    apply (fold reply_caps_mdb_def)[1]
-    apply (case_tac "sl = ptr", simp)
-    apply (simp add: fun_upd_def split del: if_split del: split_paired_Ex)
-    apply (erule allEI, rule impI, erule(1) impE)
-    apply (erule exEI)
-    apply (simp, rule ccontr)
-    apply (erule(5) emptyable_no_reply_cap)
-    apply simp
-   apply (unfold reply_masters_mdb_def)[1]
-   apply (elim allEI)
-   apply (clarsimp simp: mdb_empty_abs.descendants)
-  apply (rule conjI)
    apply (simp add: valid_ioc_def)
   apply (rule conjI)
-   apply (clarsimp simp: tcb_cap_valid_def
-                  dest!: emptyable_valid_NullCapD)
+   apply (fastforce simp: tcb_cap_valid_def
+                  dest!: valid_NullCapD)
   apply (rule conjI)
    apply (clarsimp simp: mdb_cte_at_def cte_wp_at_caps_of_state)
    apply (cases sl)
@@ -312,6 +293,9 @@ lemma length_and_unat_of_bl_length:
   "(length xs = x \<and> unat (of_bl xs :: 'a::len word) < 2 ^ x) = (length xs = x)"
   by (auto simp: unat_of_bl_length)
 
+lemmas unbind_from_sc_final_cap[wp] =
+    final_cap_lift [OF unbind_from_sc_caps_of_state]
+
 lemma (* finalise_cap_cases1 *)[Finalise_AI_asms]:
   "\<lbrace>\<lambda>s. final \<longrightarrow> is_final_cap' cap s
          \<and> cte_wp_at ((=) cap) slot s\<rbrace>
@@ -329,16 +313,17 @@ lemma (* finalise_cap_cases1 *)[Finalise_AI_asms]:
         \<and> fst_cte_ptrs (fst rv) = fst_cte_ptrs cap
         \<and> vs_cap_ref cap = None\<rbrace>"
   apply (cases cap, simp_all split del: if_split cong: if_cong)
-            apply ((wp suspend_final_cap[where sl=slot]
+            apply ((wp suspend_final_cap[where sl=slot] get_simple_ko_wp
                       deleting_irq_handler_final[where slot=slot]
                       | simp add: o_def is_cap_simps fst_cte_ptrs_def
                                   dom_tcb_cap_cases_lt_ARCH tcb_cnode_index_def
                                   can_fast_finalise_def length_and_unat_of_bl_length
                                   appropriate_cte_cap_def gen_obj_refs_def
                                   vs_cap_ref_def cap_cleanup_opt_def
-                      | intro impI TrueI ext conjI)+)[11]
+                      | intro impI TrueI ext conjI)+)[13]
   apply (simp add: arch_finalise_cap_def split del: if_split)
-  apply (wpsimp simp: cap_cleanup_opt_def arch_cap_cleanup_opt_def)
+  apply (rule hoare_pre)
+   apply (wpsimp simp: cap_cleanup_opt_def arch_cap_cleanup_opt_def)+
   done
 
 crunch typ_at_arch [wp]: arch_thread_set "\<lambda>s. P (typ_at T p s)"
@@ -453,10 +438,6 @@ lemma arch_thread_set_valid_global_refs[wp]:
   "\<lbrace>valid_global_refs\<rbrace> arch_thread_set p v \<lbrace>\<lambda>rv. valid_global_refs\<rbrace>"
   by (rule valid_global_refs_cte_lift) wp+
 
-lemma arch_thread_set_valid_reply_masters[wp]:
-  "\<lbrace>valid_reply_masters\<rbrace> arch_thread_set p v \<lbrace>\<lambda>rv. valid_reply_masters\<rbrace>"
-  by (rule valid_reply_masters_cte_lift) wp
-
 lemma arch_thread_set_pred_tcb_at[wp_unsafe]:
   "\<lbrace>pred_tcb_at proj P t and K (proj_not_field proj tcb_arch_update)\<rbrace>
      arch_thread_set p v
@@ -466,11 +447,6 @@ lemma arch_thread_set_pred_tcb_at[wp_unsafe]:
   apply (clarsimp simp: pred_tcb_at_def obj_at_def get_tcb_rev
                   dest!: get_tcb_SomeD)
   done
-
-lemma arch_thread_set_valid_reply_caps[wp]:
-  "\<lbrace>valid_reply_caps\<rbrace> arch_thread_set p v \<lbrace>\<lambda>rv. valid_reply_caps\<rbrace>"
-  by (rule valid_reply_caps_st_cte_lift)
-     (wpsimp wp: arch_thread_set_pred_tcb_at)+
 
 lemma arch_thread_set_if_unsafe_then_cap[wp]:
   "\<lbrace>if_unsafe_then_cap\<rbrace> arch_thread_set p v \<lbrace>\<lambda>rv. if_unsafe_then_cap\<rbrace>"
@@ -788,33 +764,33 @@ lemma delete_asid_unreachable:
   apply (clarsimp simp: obj_at_def in_omonad)
   done
 
-lemma arch_finalise_cap_replaceable:
-  notes strg = tcb_cap_valid_imp_NullCap
-               obj_at_not_live_valid_arch_cap_strg[where cap=cap]
+(* FIXME: move to ArchInvariants or similar *)
+lemma FrameCap_data_at:
+  "s \<turnstile> ArchObjectCap (FrameCap r R vmsz d m) \<Longrightarrow> data_at vmsz r s"
+  by (simp add: valid_cap_def obj_at_def data_at_def split: if_splits)
+
+lemma arch_finalise_cap_replaceable[wp]:
   notes simps = replaceable_def and_not_not_or_imp
-                is_cap_simps vs_cap_ref_def
+                is_cap_simps vs_cap_ref_def tcb_cap_valid_imp_NullCap
                 no_cap_to_obj_with_diff_ref_Null o_def
                 reachable_frame_cap_simps
   notes wps = hoare_drop_imp[where R="%_. is_final_cap' cap" for cap]
-              valid_cap_typ
-              unmap_page_unreachable unmap_page_table_unreachable
+              valid_cap_typ  unmap_page_unreachable unmap_page_table_unreachable
               delete_asid_unreachable
   shows
-    "\<lbrace>\<lambda>s. s \<turnstile> ArchObjectCap cap \<and>
-          x = is_final_cap' (ArchObjectCap cap) s \<and>
+    "\<lbrace>\<lambda>s. s \<turnstile> cap.ArchObjectCap cap \<and>
+          x = is_final_cap' (cap.ArchObjectCap cap) s \<and>
           pspace_aligned s \<and> valid_vspace_objs s \<and> valid_objs s \<and> valid_asid_table s \<and>
           valid_arch_caps s\<rbrace>
      arch_finalise_cap cap x
-     \<lbrace>\<lambda>rv s. replaceable s sl (fst rv) (ArchObjectCap cap)\<rbrace>"
-  apply (simp add: arch_finalise_cap_def valid_arch_caps_def)
-  apply (wpsimp simp: simps valid_objs_caps wp: wps | strengthen strg)+
-  apply (rule conjI, clarsimp)
-   apply (clarsimp simp: valid_cap_def)
-  apply (rule conjI; clarsimp)
-   apply (rule conjI; clarsimp simp: valid_cap_def wellformed_mapdata_def data_at_def split: if_split_asm)
-  apply (rule conjI; clarsimp)
-  apply (clarsimp simp: valid_cap_def wellformed_mapdata_def cap_aligned_def)
-  done
+   \<lbrace>\<lambda>rv s. replaceable s sl (fst rv) (cap.ArchObjectCap cap)\<rbrace>"
+  apply (simp add: arch_finalise_cap_def simps split: option.splits vmpage_size.splits)
+  apply (wp wps |
+         strengthen obj_at_not_live_valid_arch_cap_strg[where cap=cap] |
+         simp add: simps |
+         wpc)+
+  by (clarsimp simp: valid_objs_caps valid_arch_caps_def valid_cap_def wellformed_mapdata_def data_at_def
+      | rule conjI)+
 
 
 global_naming Arch
@@ -892,12 +868,424 @@ lemma prepare_thread_delete_unlive[wp]:
   apply (rule_tac Q="\<lambda>rv. obj_at (Not \<circ> live0) ptr and obj_at (Not \<circ> hyp_live) ptr" in hoare_strengthen_post)
   apply (wpsimp wp: hoare_vcg_conj_lift prepare_thread_delete_unlive_hyp prepare_thread_delete_unlive0)
    apply (clarsimp simp: obj_at_def)
-  apply (clarsimp simp: obj_at_def, case_tac ko, simp_all add: is_tcb_def live_def)
+  apply (clarsimp simp: obj_at_def live_def)
+  apply (auto split: kernel_object.splits)
   done
 
-lemma (* finalise_cap_replaceable *) [Finalise_AI_asms]:
-  "\<lbrace>\<lambda>s. s \<turnstile> cap \<and> x = is_final_cap' cap s \<and> valid_mdb s
-        \<and> cte_wp_at ((=) cap) sl s \<and> valid_objs s \<and> sym_refs (state_refs_of s)
+lemma sched_context_donate_bound_sc_tcb_at_None:
+  "\<lbrace>bound_sc_tcb_at ((=) None) t and K (caller_tcb \<noteq> t)\<rbrace>
+          sched_context_donate sc_ptr caller_tcb
+   \<lbrace>\<lambda>_. bound_sc_tcb_at ((=) None) t\<rbrace>"
+  apply (clarsimp simp: sched_context_donate_def)
+  apply (rule hoare_seq_ext[OF _ gsct_sp])
+  apply (wpsimp simp: sched_context_donate_def wp: ssc_bound_tcb_at_cases hoare_vcg_imp_lift')
+  done
+
+lemma set_thread_state_not_live:
+  "\<lbrace>bound_tcb_at ((=) None) t and bound_sc_tcb_at ((=) None) t
+    and bound_yt_tcb_at ((=) None) t\<rbrace>
+   set_thread_state t Inactive
+   \<lbrace>\<lambda>rv. obj_at (Not \<circ> live) t\<rbrace>"
+  by (wpsimp simp: set_thread_state_def obj_at_def pred_tcb_at_def get_tcb_def live_def hyp_live_def
+             wp: set_object_wp)
+
+lemma reply_remove_tcb_bound_sc_tcb_at_None[wp]:
+  "\<lbrace>bound_sc_tcb_at ((=) None) t'\<rbrace> reply_remove_tcb t r \<lbrace>\<lambda>rv. bound_sc_tcb_at ((=) None) t'\<rbrace>"
+  by (wpsimp simp: reply_remove_tcb_def wp: get_sk_obj_ref_wp gts_wp)
+
+lemma cancel_ipc_bound_sc_tcb_at_None:
+  "\<lbrace>bound_sc_tcb_at ((=) None) t'\<rbrace> cancel_ipc t \<lbrace>\<lambda>rv. bound_sc_tcb_at ((=) None) t'\<rbrace>"
+  by (wpsimp simp: cancel_ipc_def
+               wp: get_sk_obj_ref_wp gts_wp thread_set_no_change_tcb_pred hoare_drop_imps)
+
+lemma sched_context_cancel_yield_to_unlive:
+  "\<lbrace>bound_tcb_at ((=) None) t and bound_sc_tcb_at ((=) None) t and st_tcb_at ((=) Inactive) t\<rbrace>
+   sched_context_cancel_yield_to t
+   \<lbrace>\<lambda>_. obj_at (Not \<circ> live) t\<rbrace>"
+  apply (clarsimp simp: sched_context_cancel_yield_to_def)
+  apply (rule hoare_seq_ext[OF _ gyt_sp])
+  apply (wpsimp simp: set_tcb_obj_ref_def set_object_def update_sched_context_def
+                      get_object_def pred_tcb_at_def obj_at_def get_tcb_def live_def hyp_live_def)
+  done
+
+lemma suspend_unlive':
+  "\<lbrace>bound_tcb_at ((=) None) t and bound_sc_tcb_at ((=) None) t\<rbrace>
+   suspend t
+   \<lbrace>\<lambda>rv. obj_at (Not \<circ> live) t\<rbrace>"
+  unfolding suspend_def
+  apply (simp flip: bind_assoc)
+  apply (rule hoare_seq_ext[OF sched_context_cancel_yield_to_unlive])
+  apply (simp add: bind_assoc)
+  apply (wpsimp wp: get_object_wp cancel_ipc_bound_sc_tcb_at_None)
+  done
+
+lemma unbind_maybe_notification_not_live_helper:
+  "\<lbrace>obj_at (\<lambda>ko. \<exists>ntfn. ko = Notification ntfn \<and> ntfn_sc ntfn = None) ptr\<rbrace>
+   unbind_maybe_notification ptr
+   \<lbrace>\<lambda>rv. obj_at (\<lambda>ko. \<exists>ntfn. ko = Notification ntfn \<and>
+                                 ntfn_bound_tcb ntfn = None \<and>
+                                 ntfn_sc ntfn = None) ptr\<rbrace>"
+  apply (simp add: unbind_maybe_notification_def maybeM_def get_sk_obj_ref_def)
+  apply (rule hoare_pre)
+   apply (wp get_simple_ko_wp sbn_obj_at_impossible simple_obj_set_prop_at
+            | wpc
+            | simp add: update_sk_obj_ref_def)+
+  apply (clarsimp simp: obj_at_def)
+  done
+
+lemma sched_context_maybe_unbind_ntfn_not_bound_sc:
+  "\<lbrace>ntfn_at ptr\<rbrace> sched_context_maybe_unbind_ntfn ptr
+   \<lbrace>\<lambda>y. obj_at (\<lambda>ko. \<exists>ntfn. ko = Notification ntfn \<and>
+                        ntfn_sc ntfn = None) ptr\<rbrace>"
+    apply (simp add: sched_context_maybe_unbind_ntfn_def maybeM_def get_sk_obj_ref_def)
+  apply (rule hoare_pre)
+   apply (wp get_simple_ko_wp update_sched_context_obj_at_impossible simple_obj_set_prop_at
+             | wpc
+             | simp add: update_sk_obj_ref_def)+
+  apply (clarsimp simp: obj_at_def)
+  done
+
+lemma sc_unbind_not_live_helper:
+  "\<lbrace>ntfn_at ptr\<rbrace>
+       do sched_context_maybe_unbind_ntfn ptr;
+           unbind_maybe_notification ptr
+       od
+   \<lbrace>\<lambda>rv. obj_at (\<lambda>ko. \<exists>ntfn. ko = Notification ntfn \<and>
+                                 ntfn_bound_tcb ntfn = None \<and>
+                                 ntfn_sc ntfn = None) ptr\<rbrace>"
+  by (wpsimp wp: unbind_maybe_notification_not_live_helper sched_context_maybe_unbind_ntfn_not_bound_sc)
+
+lemma reply_unlink_sc_not_live:
+  "\<lbrace>obj_at (\<lambda>ko. \<exists>r. ko = Reply r \<and> reply_tcb r = None) reply and invs\<rbrace>
+     reply_unlink_sc sc_ptr reply
+   \<lbrace>\<lambda>rv. obj_at (\<lambda>ko. \<not> live ko \<and> is_reply ko) reply\<rbrace>"
+  apply (wpsimp wp: update_sched_context_obj_at_impossible
+                    simple_obj_set_prop_at get_simple_ko_wp
+                    set_simple_ko_obj_at_disjoint hoare_vcg_all_lift
+              simp: reply_unlink_sc_def is_reply update_sk_obj_ref_def
+        | wp (once) hoare_drop_imps)+
+  apply (clarsimp simp: obj_at_def live_def live_reply_def invs_reply_tcb_None_reply_sc_None)
+  done
+
+lemma reply_unlink_tcb_not_live:
+  "\<lbrace>reply_sc_reply_at (\<lambda>sc. sc = None) reply\<rbrace>
+     reply_unlink_tcb t reply
+   \<lbrace>\<lambda>rv. obj_at (\<lambda>ko. \<not> live ko \<and> is_reply ko) reply\<rbrace>"
+  apply (rule hoare_strengthen_post[where Q="\<lambda>rv. obj_at (\<lambda>ko. \<not> live ko \<and> is_reply ko) reply"])
+  apply (wpsimp wp: sts_obj_at_impossible update_sk_obj_ref_wps gts_wp get_simple_ko_wp
+              simp: reply_unlink_tcb_def is_reply)
+  by (auto simp: reply_sc_reply_at_def obj_at_def live_def live_reply_def)
+
+lemma not_live_reply_weaken:
+  assumes "\<lbrace>P\<rbrace> f \<lbrace>\<lambda>rv. obj_at (\<lambda>ko. \<not> live ko \<and> is_reply ko) reply\<rbrace>"
+  shows "\<lbrace>P\<rbrace> f \<lbrace>\<lambda>rv. obj_at (Not \<circ> live) reply\<rbrace>"
+  by (rule hoare_strengthen_post[OF assms], erule obj_at_weakenE, simp)
+
+lemma reply_unlink_sc_None:
+  "\<lbrace>reply_at reply and valid_objs\<rbrace>
+       reply_unlink_sc scp reply
+   \<lbrace>\<lambda>rv. reply_sc_reply_at (\<lambda>sc. sc = None) reply\<rbrace>"
+  apply (clarsimp simp: reply_unlink_sc_def reply_sc_reply_at_def)
+  apply (wpsimp simp: is_reply update_sk_obj_ref_def
+               wp: update_sched_context_obj_at_impossible simple_obj_set_prop_at get_simple_ko_wp
+                   set_simple_ko_obj_at_disjoint hoare_vcg_all_lift assert_wp hoare_vcg_const_imp_lift
+        | wp (once) hoare_drop_imps)+
+  apply (rule conjI, clarsimp)
+   apply (erule_tac p=scp in obj_at_valid_objsE, assumption)
+   apply (clarsimp simp: valid_obj_def valid_sched_context_def dest!:distinct_hd_not_in_tl)
+  apply (clarsimp simp: obj_at_def)
+  done
+
+lemma sc_with_reply_None_no_reply_sc:
+  "\<lbrakk>kheap s rp' = Some (Reply reply); invs s; sc_with_reply rp' s = None\<rbrakk>
+       \<Longrightarrow> reply_sc reply = None"
+  apply (rule ccontr, clarsimp simp: obj_at_def)
+  apply (drule(3) reply_sc_refs[OF _ invs_valid_objs invs_sym_refs])
+  apply (drule_tac sc=y in valid_replies_sc_with_reply_None[OF _ invs_valid_replies])
+   apply (clarsimp simp: sc_at_ppred_def obj_at_def)+
+  done
+
+lemma reply_remove_unlive:
+  "\<lbrace>invs and K (rp = rp')\<rbrace>
+     reply_remove t rp
+   \<lbrace>\<lambda>rv. obj_at (Not \<circ> live) rp'\<rbrace>"
+  supply if_split[split del]
+  apply (simp add: reply_remove_def assert_opt_def)
+  apply (rule hoare_gen_asm[simplified])
+  apply (rule hoare_seq_ext[OF _ get_simple_ko_sp])
+  apply (rule hoare_seq_ext[OF _ assert_sp, OF hoare_gen_asm_conj], clarsimp)
+  apply (rule hoare_seq_ext[OF _ gets_sp])
+  apply (wpsimp wp: not_live_reply_weaken[OF reply_unlink_tcb_not_live] reply_unlink_sc_None)
+  by (clarsimp simp: reply_sc_reply_at_def obj_at_def is_reply invs_valid_objs
+                     sc_with_reply_None_no_reply_sc)
+
+lemma reply_unlink_tcb_not_live':
+  "\<lbrace>reply_sc_reply_at (\<lambda>sc. sc = None) reply and K (reply = reply')\<rbrace>
+   reply_unlink_tcb t reply'
+   \<lbrace>\<lambda>rv. obj_at (Not \<circ> live) reply\<rbrace>"
+  by (rule hoare_gen_asm)
+     (wpsimp wp: not_live_reply_weaken[OF reply_unlink_tcb_not_live] simp: obj_at_def)
+
+lemma st_tcb_recv_reply_state_refs:
+  "\<lbrakk>valid_objs s; sym_refs (state_refs_of s); st_tcb_at ((=) (BlockedOnReceive ep (Some reply) pl)) thread s\<rbrakk>
+  \<Longrightarrow> \<exists>rep. (kheap s reply = Some (Reply rep) \<and> reply_tcb rep = Some thread)"
+  apply (frule (1) st_tcb_at_valid_st2)
+  apply (drule (1) sym_refs_st_tcb_atD[rotated])
+  apply (clarsimp simp: get_refs_def2 obj_at_def valid_tcb_state_def is_reply
+                  split: thread_state.splits if_splits)
+  done
+
+lemma blocked_cancel_ipc_unlive:
+  "\<lbrace>st_tcb_at ((=) st) thread and (\<lambda>s. sym_refs (state_refs_of s)) and valid_replies and valid_objs
+    and K (rep = Some reply \<and> (\<exists>ep pl. st = BlockedOnReceive ep rep pl))\<rbrace>
+    blocked_cancel_ipc st thread rep
+   \<lbrace>\<lambda>rv. obj_at (Not \<circ> live) reply\<rbrace>"
+  apply (rule hoare_gen_asm, clarsimp)
+  apply (rule_tac Q="\<lambda>rv. obj_at (\<lambda>ko. \<not>live ko \<and> is_reply ko) reply" in hoare_strengthen_post[rotated]
+         , fastforce simp: obj_at_def)
+  apply (simp add: blocked_cancel_ipc_def)
+  apply (rule hoare_seq_ext[OF _ gbi_ep_sp])
+  by (wpsimp wp: sts_obj_at_impossible reply_unlink_tcb_not_live
+                 get_simple_ko_wp hoare_vcg_all_lift
+           simp: is_reply reply_sc_reply_at_def obj_at_def)
+     (fastforce dest!: valid_replies_ReceiveD[simplified reply_sc_reply_at_def obj_at_def])
+
+lemma cancel_ipc_unlive_reply_receive:
+  "\<lbrace> (\<lambda>s. sym_refs (state_refs_of s)) and valid_replies and valid_objs
+     and st_tcb_at (\<lambda>st. (\<exists>x pl. st = (BlockedOnReceive x (Some reply) pl))) thread\<rbrace>
+     cancel_ipc thread
+   \<lbrace>\<lambda> rv. obj_at (Not \<circ> live) reply\<rbrace>"
+  apply (clarsimp simp: cancel_ipc_def)
+  apply wpsimp
+         apply (rule blocked_cancel_ipc_unlive)
+        apply (rule hoare_pre_cont)
+       apply (rule hoare_pre_cont)
+      apply (rule hoare_pre_cont)
+     apply (wpsimp wp: thread_set_wp gts_wp)+
+  apply (clarsimp simp: get_tcb_ko_at pred_tcb_at_def obj_at_def
+                        state_refs_of_tcb_fault_update
+                        valid_replies_tcb_fault_update)
+  apply (rule valid_objs_same_type, simp)
+   apply (clarsimp simp: a_type_def obj_at_def)
+  apply (erule (1) valid_objsE)
+  by (clarsimp simp: valid_obj_def valid_tcb_def valid_objs_def ran_tcb_cap_cases)
+
+lemma reply_unlink_sc_not_live':
+ "\<lbrace>obj_at (\<lambda>ko. \<exists>r. ko = Reply r \<and> reply_tcb r = None) reply and invs\<rbrace>
+    reply_unlink_sc sc_ptr reply
+  \<lbrace>\<lambda>rv. obj_at (Not \<circ> live) reply\<rbrace>"
+  by (rule hoare_strengthen_post, rule reply_unlink_sc_not_live, clarsimp simp: obj_at_def)
+
+lemma set_tcb_yt_update_bound_tcb_at[wp]:
+  "set_tcb_obj_ref tcb_yield_to_update scp tcb \<lbrace>bound_tcb_at P t\<rbrace>"
+  by (wpsimp simp: set_tcb_obj_ref_def pred_tcb_at_def obj_at_def get_tcb_rev wp: set_object_wp)
+
+lemma complete_yield_to_bound_tcb_at[wp]:
+  "\<lbrace>bound_tcb_at P t\<rbrace> complete_yield_to scptr \<lbrace>\<lambda>rv. bound_tcb_at P t\<rbrace>"
+  by (wpsimp simp: complete_yield_to_def set_consumed_def get_sc_obj_ref_def
+               wp: set_thread_state_bound_tcb_at set_message_info_st_tcb_at hoare_drop_imp)
+
+lemma complete_yield_to_bound_sc_tcb_at[wp]:
+  "\<lbrace>bound_sc_tcb_at P t\<rbrace> complete_yield_to scptr \<lbrace>\<lambda>rv. bound_sc_tcb_at P t\<rbrace>"
+  by (wpsimp simp: complete_yield_to_def set_consumed_def get_sc_obj_ref_def
+               wp: set_thread_state_bound_sc_tcb_at set_message_info_st_tcb_at hoare_drop_imp)
+
+lemma ssc_bound_yt_tcb_at[wp]:
+  "\<lbrace>bound_yt_tcb_at P t\<rbrace> set_tcb_obj_ref tcb_sched_context_update tcb ntfn \<lbrace>\<lambda>_. bound_yt_tcb_at P t\<rbrace>"
+  apply (simp add: set_tcb_obj_ref_def)
+  apply (wp set_object_wp)
+  apply (auto simp: pred_tcb_at_def obj_at_def get_tcb_def)
+  done
+
+lemma sched_context_unbind_tcb_bound_tcb_at[wp]:
+  "\<lbrace>bound_tcb_at P t\<rbrace> sched_context_unbind_tcb a \<lbrace>\<lambda>y. bound_tcb_at P t\<rbrace>"
+  by (wpsimp simp: sched_context_unbind_tcb_def wp: get_sched_context_wp)
+
+lemma sched_context_unbind_tcb_bound_yt_tcb_at[wp]:
+  "\<lbrace>bound_yt_tcb_at P t\<rbrace> sched_context_unbind_tcb a \<lbrace>\<lambda>y. bound_yt_tcb_at P t\<rbrace>"
+  by (wpsimp simp: sched_context_unbind_tcb_def wp: get_sched_context_wp)
+
+lemma unbind_from_sc_bound_tcb_at[wp]:
+  "\<lbrace>bound_tcb_at P t\<rbrace> unbind_from_sc x \<lbrace>\<lambda>rv. bound_tcb_at P t\<rbrace>"
+  by (wpsimp simp: unbind_from_sc_def wp: hoare_drop_imps hoare_vcg_all_lift)
+
+lemma sched_context_unbind_tcb_bound_sc_tcb_at_None:
+  "\<lbrace>\<lambda>s. obj_at (\<lambda>obj. \<exists>n na. obj = SchedContext n na \<and> sc_tcb n = Some tcbptr) sc s \<rbrace>
+         sched_context_unbind_tcb sc
+   \<lbrace>\<lambda>_. bound_sc_tcb_at ((=) None) tcbptr\<rbrace>"
+  apply (simp add: sched_context_unbind_tcb_def maybeM_def)
+  apply (wpsimp wp: ssc_bound_tcb_at_cases get_sched_context_wp hoare_vcg_const_imp_lift)
+  apply (clarsimp simp: obj_at_def)
+  done
+
+lemma unbind_from_sc_bound_sc_tcb_at:
+  "\<lbrace>tcb_at x and valid_objs and (\<lambda>s. sym_refs (state_refs_of s))\<rbrace>
+     unbind_from_sc x
+   \<lbrace>\<lambda>rv. bound_sc_tcb_at ((=) None) x\<rbrace>"
+  apply (simp add: unbind_from_sc_def)
+    apply (wpsimp wp: sched_context_unbind_tcb_bound_sc_tcb_at_None
+                      hoare_vcg_all_lift gbn_wp
+           | wp (once) hoare_drop_imps)+
+  apply (clarsimp simp: obj_at_def is_tcb pred_tcb_at_def)
+  apply (erule(1) pspace_valid_objsE)
+  by (auto simp: obj_at_def pred_tcb_at_def valid_obj_def valid_tcb_def
+                 sc_at_typ typ_at_eq_kheap_obj
+          dest!: bound_sc_tcb_bound_sc_at)
+
+lemma complete_yield_to_unbinds:
+  "\<lbrace>tcb_at t\<rbrace>
+     complete_yield_to t
+   \<lbrace>\<lambda>rv. bound_yt_tcb_at ((=) None) t\<rbrace>"
+  apply (clarsimp simp: complete_yield_to_def)
+  apply (wpsimp simp: complete_yield_to_def wp: syt_bound_tcb_at' maybeM_wp gbn_wp)
+  apply (clarsimp simp: obj_at_def pred_tcb_at_def is_tcb)
+  done
+
+lemma bound_yt_tcb_bound_yield_from_at:
+  "\<lbrakk>sym_refs (state_refs_of s); valid_objs s; kheap s scptr = Some (SchedContext sc a);
+    bound_yt_tcb_at (\<lambda>ptr. ptr = (Some scptr)) tcbptr s \<rbrakk>
+  \<Longrightarrow> sc_yield_from sc = Some tcbptr"
+  apply (drule_tac x=tcbptr in sym_refsD[rotated])
+   apply (fastforce simp: state_refs_of_def pred_tcb_at_def obj_at_def)
+  apply (auto simp: pred_tcb_at_def obj_at_def valid_obj_def valid_sched_context_def is_tcb
+                    state_refs_of_def refs_of_rev
+          simp del: refs_of_simps)
+  done
+
+lemma unbind_from_sc_no_cap_to_obj_ref[wp]:
+  "\<lbrace>no_cap_to_obj_with_diff_ref cap S\<rbrace>
+     unbind_from_sc tcbptr
+   \<lbrace>\<lambda>_. no_cap_to_obj_with_diff_ref cap S\<rbrace>"
+  apply (simp add: no_cap_to_obj_with_diff_ref_def cte_wp_at_caps_of_state)
+  apply (wp)
+  done
+
+lemma set_sc_obj_ref_not_live:
+  "\<lbrace>obj_at (\<lambda>ko. \<exists>sc n. ko = SchedContext sc n \<and> sc_tcb sc = None
+                        \<and> sc_ntfn sc = None \<and> sc_replies sc = []) sc
+    and K (t = sc)\<rbrace>
+     set_sc_obj_ref sc_yield_from_update t None
+   \<lbrace>\<lambda>_. obj_at (Not \<circ> live) sc\<rbrace>"
+  supply if_split[split del]
+  by (wpsimp simp: update_sched_context_def set_object_def
+                   get_sched_context_def obj_at_def live_def live_sc_def
+               wp: get_object_wp)
+
+lemma complete_yield_to_not_live:
+  "\<lbrace>obj_at (\<lambda>ko. \<exists>sc n. ko = SchedContext sc n \<and> sc_yield_from sc = Some tcb
+                        \<and> sc_tcb sc = None \<and> sc_ntfn sc = None \<and> sc_replies sc = []) sc
+    and valid_objs and (\<lambda>s. sym_refs (state_refs_of s))\<rbrace>
+     complete_yield_to tcb
+   \<lbrace>\<lambda>yc a. obj_at (Not \<circ> live) sc a\<rbrace>"
+  apply (clarsimp simp: complete_yield_to_def get_tcb_obj_ref_def)
+  apply (wpsimp wp: thread_get_wp' set_sc_obj_ref_not_live
+                    set_tcb_obj_ref_obj_at_trivial
+                    set_consumed_obj_at_trivial
+                    get_object_wp hoare_vcg_all_lift
+         | wp (once) hoare_drop_imps)+
+  apply (auto simp: obj_at_def live_def live_sc_def dest: sym_ref_sc_yf)
+  done
+
+lemma sched_context_unbind_yield_from_not_live:
+  "\<lbrace>obj_at (\<lambda>ko. \<exists>sc n. ko = SchedContext sc n \<and> sc_tcb sc = None
+                        \<and> sc_ntfn sc = None \<and> sc_replies sc = []) sc
+     and invs\<rbrace>
+   sched_context_unbind_yield_from sc
+   \<lbrace>\<lambda>yc a. obj_at (Not \<circ> live) sc a\<rbrace>"
+  apply (clarsimp simp: sched_context_unbind_yield_from_def)
+  apply (wpsimp wp: complete_yield_to_not_live)
+  apply (auto simp: obj_at_def live_def live_sc_def)
+  done
+
+lemma sc_refill_max_update_not_live[wp]:
+  "update_sched_context sc_ptr (sc_refill_max_update f) \<lbrace>obj_at (Not \<circ> live) sc\<rbrace>"
+  apply (wpsimp simp: wp: update_sched_context_wp)
+  apply (auto simp: obj_at_def live_def live_sc_def)
+  done
+
+method hammer = ((clarsimp simp: o_def dom_tcb_cap_cases_lt_ARCH
+                                 ran_tcb_cap_cases is_cap_simps
+                                 cap_range_def prepare_thread_delete_def
+                                 can_fast_finalise_def
+                                 gen_obj_refs_subset
+                                 vs_cap_ref_def
+                                 valid_ipc_buffer_cap_def valid_fault_handler_def
+                           dest!: tcb_cap_valid_NullCapD
+                           split: Structures_A.thread_state.split_asm
+                   | simp cong: conj_cong
+                   | simp cong: rev_conj_cong add: no_cap_to_obj_with_diff_ref_Null
+                   | (strengthen tcb_cap_valid_imp_NullCap tcb_cap_valid_imp', wp)
+                   | erule cte_wp_at_weakenE tcb_cap_valid_imp'[rule_format, rotated -1]
+                   | erule(1) no_cap_to_obj_with_diff_ref_finalI_ARCH
+                   | ((wp (once) hoare_drop_imps)?,
+                      (wp (once) hoare_drop_imps)?,
+                      wp (once) deleting_irq_handler_empty)
+                   | simp add: valid_cap_simps)+)[1]
+
+lemma sched_context_unbind_ntfn_unbinds:
+  "\<lbrace>obj_at (\<lambda>ko. \<exists>sc n. ko = SchedContext sc n \<and> sc_tcb sc = None) sc \<rbrace>
+      sched_context_unbind_ntfn sc
+   \<lbrace>\<lambda>rv. obj_at (\<lambda>ko. \<exists>sc. (\<exists>n. ko = SchedContext sc n) \<and> sc_tcb sc = None \<and> sc_ntfn sc = None) sc\<rbrace>"
+  unfolding sched_context_unbind_ntfn_def
+  apply (wpsimp simp: update_sched_context_def set_object_def update_sk_obj_ref_def
+                      set_simple_ko_def get_sc_obj_ref_def
+                  wp: get_object_wp get_simple_ko_wp )
+  by (auto simp: obj_at_def)
+
+lemma sched_context_unbind_ntfn_valid_objs[wp]:
+  notes refs_of_simps[simp del]
+  shows
+  "\<lbrace>valid_objs\<rbrace> sched_context_unbind_ntfn sc \<lbrace>\<lambda>rv. valid_objs\<rbrace>"
+  apply (simp add: sched_context_unbind_ntfn_def get_sc_obj_ref_def)
+  apply (wpsimp simp: update_sk_obj_ref_def
+                  wp: valid_irq_node_typ set_simple_ko_valid_objs get_simple_ko_wp get_sched_context_wp
+                      valid_ioports_lift)
+  apply (clarsimp simp: obj_at_def is_ntfn sc_ntfn_sc_at_def)
+  apply (frule valid_objs_valid_sched_context_size, fastforce)
+  apply (erule_tac x=x in valid_objsE, simp)
+  apply (clarsimp simp: valid_obj_def valid_ntfn_def obj_at_def is_sc_obj_def split: ntfn.splits)
+  done
+
+lemma sched_context_unbind_ntfn_sym_refs[wp]:
+  notes refs_of_simps[simp del]
+  shows
+  "\<lbrace>\<lambda>s. valid_objs s \<and> sym_refs (state_refs_of s)\<rbrace> sched_context_unbind_ntfn sc \<lbrace>\<lambda>rv s. sym_refs (state_refs_of s) \<rbrace>"
+  apply (simp add: sched_context_unbind_ntfn_def get_sc_obj_ref_def)
+  apply (wpsimp simp: update_sk_obj_ref_def
+                  wp: valid_irq_node_typ set_simple_ko_valid_objs get_simple_ko_wp get_sched_context_wp
+                      valid_ioports_lift)
+  apply (clarsimp simp: obj_at_def is_ntfn sc_ntfn_sc_at_def)
+  apply (frule sym_refs_ko_atD[where p=sc, rotated], fastforce simp: obj_at_def)
+  apply (frule sym_refs_ko_atD[where ko="Notification x" for x, rotated], fastforce simp: obj_at_def)
+  apply (erule delta_sym_refs)
+   apply (fastforce simp: obj_at_def refs_of_simps split: if_splits)
+  by (fastforce split: if_split_asm ntfn.splits
+                dest!: symreftype_inverse'
+                 simp: obj_at_def get_refs_def2  ntfn_q_refs_of_def image_iff refs_of_simps)
+
+lemma sched_context_unbind_all_tcbs_unbinds:
+  "\<lbrace>sc_at sc and K (sc \<noteq> idle_sc_ptr)\<rbrace>
+       sched_context_unbind_all_tcbs sc
+   \<lbrace>\<lambda>y a. obj_at (\<lambda>ko. \<exists>sc. (\<exists>n. ko = SchedContext sc n) \<and> sc_tcb sc = None) sc a\<rbrace>"
+  apply (clarsimp simp: sched_context_unbind_all_tcbs_def sched_context_unbind_tcb_def)
+  apply (wpsimp simp: update_sched_context_def
+                  wp: set_object_at_obj3)
+  by (auto simp: obj_at_def)
+
+lemma finalise_cap_replaceable_helper:
+  "\<lbrace>obj_at (\<lambda>ko. \<exists>sc n. ko = SchedContext sc n \<and> sc_tcb sc = None \<and> sc_ntfn sc = None) sc \<rbrace>
+      sched_context_unbind_reply sc
+   \<lbrace>\<lambda>rv. obj_at (\<lambda>ko. \<exists>sc. (\<exists>n. ko = SchedContext sc n) \<and> sc_tcb sc = None
+                                \<and> sc_ntfn sc = None \<and> sc_replies sc = []) sc\<rbrace>"
+  unfolding sched_context_unbind_reply_def
+  apply (wpsimp simp: update_sched_context_def set_object_def update_sk_obj_ref_def
+                      set_simple_ko_def get_sc_obj_ref_def
+                  wp: get_object_wp get_simple_ko_wp )
+  by (auto simp: obj_at_def)
+
+lemma finalise_cap_replaceable [Finalise_AI_asms]:
+  "\<lbrace>\<lambda>s. s \<turnstile> cap \<and> x = is_final_cap' cap s
+        \<and> cte_wp_at ((=) cap) sl s \<and> invs s
         \<and> (cap_irqs cap \<noteq> {} \<longrightarrow> if_unsafe_then_cap s \<and> valid_global_refs s)
         \<and> (is_arch_cap cap \<longrightarrow> pspace_aligned s \<and>
                                valid_vspace_objs s \<and>
@@ -907,43 +1295,81 @@ lemma (* finalise_cap_replaceable *) [Finalise_AI_asms]:
    \<lbrace>\<lambda>rv s. replaceable s sl (fst rv) cap\<rbrace>"
   apply (cases "is_arch_cap cap")
    apply (clarsimp simp: is_cap_simps)
-   apply (wp arch_finalise_cap_replaceable)
+   apply wp
    apply (clarsimp simp: replaceable_def reachable_frame_cap_def
                          o_def cap_range_def valid_arch_state_def
                          ran_tcb_cap_cases is_cap_simps
-                         gen_obj_refs_subset vs_cap_ref_def
-                         all_bool_eq)
-  apply (cases cap;
-           simp add: replaceable_def reachable_frame_cap_def is_arch_cap_def
-                split del: if_split;
-           ((wp suspend_unlive[unfolded o_def]
-                suspend_final_cap[where sl=sl]
-                prepare_thread_delete_unlive[unfolded o_def]
-                unbind_maybe_notification_not_bound
-                get_simple_ko_ko_at
-             | clarsimp simp: o_def dom_tcb_cap_cases_lt_ARCH
-                              ran_tcb_cap_cases is_cap_simps
-                              cap_range_def unat_of_bl_length
-                              can_fast_finalise_def
-                              gen_obj_refs_subset
-                              vs_cap_ref_def
-                              valid_ipc_buffer_cap_def
-                        dest!: tcb_cap_valid_NullCapD
-                        split: Structures_A.thread_state.split_asm
-             | simp cong: conj_cong
-             | simp cong: rev_conj_cong add: no_cap_to_obj_with_diff_ref_Null
-             | (strengthen tcb_cap_valid_imp_NullCap tcb_cap_valid_imp', wp)
-             | rule conjI
-             | erule cte_wp_at_weakenE tcb_cap_valid_imp'[rule_format, rotated -1]
-             | erule(1) no_cap_to_obj_with_diff_ref_finalI_ARCH
-             | (wp (once) hoare_drop_imps,
-                        wp (once) cancel_all_ipc_unlive[unfolded o_def]
-                       cancel_all_signals_unlive[unfolded o_def])
-             | ((wp (once) hoare_drop_imps)?,
-                (wp (once) hoare_drop_imps)?,
-                wp (once) deleting_irq_handler_empty)
-             | wpc
-             | simp add: valid_cap_simps is_nondevice_page_cap_simps)+))
+                         gen_obj_refs_subset vs_cap_ref_def)
+  apply (cases cap; simp add: replaceable_def reachable_frame_cap_def
+                         split del: if_split)
+               \<comment> \<open>NullCap\<close>
+               apply (rule hoare_pre)
+                apply (wpsimp, clarsimp)
+              \<comment> \<open>untyped\<close>
+              apply (wpsimp)
+              apply hammer
+             \<comment> \<open>endpoint\<close>
+             apply ((wpsimp
+                    | hammer
+                    | (wp (once) hoare_drop_imps,
+                       wp (once) reply_unlink_sc_not_live'[unfolded o_def]
+                                 cancel_all_ipc_unlive[unfolded o_def]
+                                 cancel_all_signals_unlive[unfolded o_def]))+)[2]
+             apply fastforce
+           \<comment> \<open>ntfn\<close>
+            apply ((wpsimp wp: unbind_maybe_notification_not_live_helper sched_context_maybe_unbind_ntfn_not_bound_sc
+                    | hammer
+                    | (wp (once) hoare_drop_imps, wp (once) reply_unlink_sc_not_live'[unfolded o_def]
+                            cancel_all_ipc_unlive[unfolded o_def]
+                            cancel_all_signals_unlive[unfolded o_def]))+)[1]
+           \<comment> \<open>reply\<close>
+           apply ((wpsimp wp: unbind_maybe_notification_not_live_helper sched_context_maybe_unbind_ntfn_not_bound_sc | hammer)+)[1]
+                     apply (rename_tac tcb, rule_tac t=tcb and s= "the (reply_tcb reply)" in subst, simp)
+                     apply (wp (once) hoare_drop_imps, rule hoare_vcg_conj_lift,
+                             wp (once) cancel_ipc_unlive_reply_receive[unfolded o_def], hammer)
+                    apply ((wpsimp wp: gts_wp get_simple_ko_wp | hammer | wp (once) hoare_drop_imps, rule hoare_vcg_conj_lift,
+                             wp (once) cancel_ipc_unlive_reply_receive[unfolded o_def] reply_remove_unlive[unfolded o_def])+)[9]
+           apply (auto simp: obj_at_def is_cap_simps ran_tcb_cap_cases valid_ipc_buffer_cap_def pred_tcb_at_def
+                             live_def live_reply_def vs_cap_ref_def no_cap_to_obj_with_diff_ref_Null
+                             invs_reply_tcb_None_reply_sc_None
+                      intro: valid_NullCapD
+                      dest!: reply_tcb_state_refs)[1]
+          \<comment> \<open>Cnode\<close>
+          apply ((wpsimp | hammer)+)[1]
+          apply (rule conjI)
+           apply (clarsimp simp: obj_at_def)
+           apply (case_tac ko; clarsimp simp: is_cap_table_def[split_simps kernel_object.split] live_def)
+          apply (rule conjI, clarsimp simp: unat_of_bl_length)
+          apply (rule conjI, clarsimp)
+           apply (erule tcb_cap_valid_imp'[rule_format, rotated -1])
+           apply hammer
+          apply hammer
+         \<comment> \<open>tcb\<close>
+         apply ((wpsimp wp: suspend_final_cap suspend_unlive'[unfolded o_def]
+                            unbind_from_sc_bound_sc_tcb_at
+                 | hammer | rule conjI)+)[1]
+        \<comment> \<open>domain\<close>
+        apply ((wpsimp | hammer)+)[1]
+       \<comment> \<open>schedcontext\<close>
+       apply ((wpsimp wp: sched_context_unbind_ntfn_unbinds
+                         sched_context_unbind_all_tcbs_unbinds
+                         finalise_cap_replaceable_helper
+                   simp: no_cap_to_idle_sc_ptr
+              | hammer
+              | wp (once) sched_context_unbind_yield_from_not_live[unfolded o_def]
+              | wp (once) hoare_drop_imps; wp (once) hoare_vcg_conj_lift,
+                wp (once) sc_refill_max_update_not_live[unfolded o_def])+)[1]
+     \<comment> \<open>schedcontrol\<close>
+      apply ((wpsimp | hammer)+)[1]
+     \<comment> \<open>irqcontrol\<close>
+     apply ((wpsimp | hammer)+)[1]
+    \<comment> \<open>irqhandler\<close>
+    apply ((wpsimp | hammer)+)[1]
+    apply fastforce
+   \<comment> \<open>zombie\<close>
+   apply ((wpsimp | hammer)+)[1]
+  \<comment> \<open>arch\<close>
+  apply (clarsimp simp: is_cap_simps)
   done
 
 lemma (* deleting_irq_handler_cte_preserved *)[Finalise_AI_asms]:
@@ -964,25 +1390,24 @@ lemma arch_thread_set_cte_wp_at[wp]:
     apply (clarsimp simp: tcb_cnode_map_def)+
   done
 
-crunch cte_wp_at[wp,Finalise_AI_asms]: prepare_thread_delete "\<lambda>s. P (cte_wp_at P' p s)"
-
-crunch cte_wp_at[wp,Finalise_AI_asms]: arch_finalise_cap "\<lambda>s. P (cte_wp_at P' p s)"
+crunches prepare_thread_delete, arch_finalise_cap
+  for cte_wp_at[wp, Finalise_AI_asms]: "\<lambda>s. P (cte_wp_at P' p s)"
+  and cur[wp, Finalise_AI_asms]: "\<lambda>s. P (cur_thread s)"
   (simp: crunch_simps assertE_def wp: crunch_wps set_object_cte_at
    ignore: arch_thread_set)
+
 end
 
 interpretation Finalise_AI_1?: Finalise_AI_1
-  proof goal_cases
+proof goal_cases
   interpret Arch .
   case 1 show ?case by (intro_locales; (unfold_locales; fact Finalise_AI_asms)?)
-  qed
+qed
 
 context Arch begin global_naming RISCV64
 
 lemma fast_finalise_replaceable[wp]:
-  "\<lbrace>\<lambda>s. s \<turnstile> cap \<and> x = is_final_cap' cap s
-     \<and> cte_wp_at ((=) cap) sl s \<and> valid_asid_table s
-     \<and> valid_mdb s \<and> valid_objs s \<and> sym_refs (state_refs_of s)\<rbrace>
+  "\<lbrace>\<lambda>s. s \<turnstile> cap \<and> x = is_final_cap' cap s \<and> cte_wp_at ((=) cap) sl s \<and> invs s\<rbrace>
      fast_finalise cap x
    \<lbrace>\<lambda>rv s. cte_wp_at (replaceable s sl cap.NullCap) sl s\<rbrace>"
   apply (cases "cap_irqs cap = {}")
@@ -1000,12 +1425,12 @@ lemma fast_finalise_replaceable[wp]:
 
 global_naming Arch
 lemma (* cap_delete_one_invs *) [Finalise_AI_asms,wp]:
-  "\<lbrace>invs and emptyable ptr\<rbrace> cap_delete_one ptr \<lbrace>\<lambda>rv. invs\<rbrace>"
+  "\<lbrace>invs\<rbrace> cap_delete_one ptr \<lbrace>\<lambda>rv. invs\<rbrace>"
   apply (simp add: cap_delete_one_def unless_def is_final_cap_def)
   apply (rule hoare_pre)
-  apply (wp empty_slot_invs get_cap_wp)
-  apply clarsimp
-  apply (drule cte_wp_at_valid_objs_valid_cap, fastforce+)
+  apply (wp empty_slot_invs get_cap_wp fast_finalise_invs)
+  apply (clarsimp; intro conjI; simp?)
+   apply (drule cte_wp_at_valid_objs_valid_cap, fastforce+)
   done
 
 end
@@ -1086,8 +1511,10 @@ lemma is_arch_update_reset_page:
   apply (simp add: is_arch_update_def is_arch_cap_def cap_master_cap_def)
   done
 
+context notes if_cong[cong] begin
 crunch caps_of_state [wp]: arch_finalise_cap "\<lambda>s. P (caps_of_state s)"
    (wp: crunch_wps simp: crunch_simps)
+end
 
 lemma set_vm_root_empty[wp]:
   "\<lbrace>\<lambda>s. P (obj_at (empty_table S) p s)\<rbrace> set_vm_root v \<lbrace>\<lambda>_ s. P (obj_at (empty_table S) p s) \<rbrace>"
@@ -1156,26 +1583,32 @@ crunch invs[wp]: prepare_thread_delete invs
   (ignore: set_object)
 
 lemma (* finalise_cap_invs *)[Finalise_AI_asms]:
-  shows "\<lbrace>invs and cte_wp_at ((=) cap) slot\<rbrace> finalise_cap cap x \<lbrace>\<lambda>rv. invs\<rbrace>"
+  "\<lbrace>invs and cte_wp_at ((=) cap) slot\<rbrace> finalise_cap cap x \<lbrace>\<lambda>_ s. invs s\<rbrace>"
   apply (cases cap, simp_all split del: if_split)
-         apply (wp cancel_all_ipc_invs cancel_all_signals_invs unbind_notification_invs
-                   unbind_maybe_notification_invs
-                  | simp add: o_def split del: if_split cong: if_cong
-                  | wpc )+
-      apply clarsimp (* thread *)
-      apply (frule cte_wp_at_valid_objs_valid_cap, clarsimp)
-      apply (clarsimp simp: valid_cap_def)
-      apply (frule(1) valid_global_refsD[OF invs_valid_global_refs])
-       apply (simp add: global_refs_def, rule disjI1, rule refl)
-      apply (simp add: cap_range_def)
-     apply (wp deleting_irq_handler_invs  | simp | intro conjI impI)+
-  apply (auto dest: cte_wp_at_valid_objs_valid_cap)
+               prefer 7
+               apply (wpsimp wp: suspend_invs unbind_notification_invs)
+               apply (fastforce simp: invs_def valid_state_def valid_idle_def cap_range_def
+                               dest!: valid_global_refsD)
+              apply (wp cancel_all_ipc_invs cancel_all_signals_invs gts_wp
+                        unbind_maybe_notification_invs get_simple_ko_wp  reply_remove_invs
+                        sched_context_unbind_yield_from_invs
+                    | simp add: o_def split del: if_split cong: if_cong
+                    | wpc
+                    | solves \<open>clarsimp dest!: no_cap_to_idle_sc_ptr\<close>
+                    | solves \<open> clarsimp,
+                               (frule (2) reply_tcb_state_refs[OF _ invs_valid_objs invs_sym_refs],
+                                fastforce simp: obj_at_def, clarsimp),
+                                (auto simp: reply_tcb_reply_at_def pred_tcb_at_def obj_at_def)\<close>)+
+  apply clarsimp
+  apply (frule cte_wp_at_valid_objs_valid_cap, clarsimp)
+  apply (clarsimp simp: valid_cap_def)
   done
 
 lemma (* finalise_cap_irq_node *)[Finalise_AI_asms]:
-"\<lbrace>\<lambda>s. P (interrupt_irq_node s)\<rbrace> finalise_cap a b \<lbrace>\<lambda>_ s. P (interrupt_irq_node s)\<rbrace>"
+  "\<lbrace>\<lambda>s. P (interrupt_irq_node s)\<rbrace> finalise_cap a b \<lbrace>\<lambda>_ s. P (interrupt_irq_node s)\<rbrace>"
+  supply if_cong[cong]
   apply (case_tac a,simp_all)
-  apply (wp | clarsimp)+
+  apply (wpsimp wp: hoare_drop_imps| clarsimp)+
   done
 
 lemmas (*arch_finalise_cte_irq_node *) [wp,Finalise_AI_asms]
@@ -1261,9 +1694,11 @@ lemma (* dmo_replaceable_or_arch_update *) [Finalise_AI_asms,wp]:
   \<lbrace>\<lambda>r s. replaceable_or_arch_update s slot cap cap'\<rbrace>"
   unfolding replaceable_or_arch_update_def replaceable_def no_cap_to_obj_with_diff_ref_def
             replaceable_final_arch_cap_def replaceable_non_final_arch_cap_def
-  apply (wp_pre, wps dmo_tcb_cap_valid_ARCH do_machine_op_reachable_pg_cap)
-   apply (rule hoare_vcg_prop)
-  apply simp
+  supply if_cong[cong]
+  apply (rule hoare_pre)
+  apply (wps dmo_tcb_cap_valid_ARCH do_machine_op_reachable_pg_cap)
+  apply (rule hoare_vcg_prop)
+  apply auto
   done
 
 end
@@ -1347,7 +1782,7 @@ lemma valid_idle_has_null_cap_ARCH[Finalise_AI_asms]:
   apply (case_tac capa, simp_all add: cap_range_def global_refs_def)[1]
   apply (clarsimp simp: valid_irq_node_def valid_idle_def pred_tcb_at_def
                         obj_at_def is_cap_table_def)
-  apply (rename_tac word tcb)
+  apply (rename_tac word tcb sc)
   apply (drule_tac x=word in spec, simp)
   done
 
