proof/invariant-abstract/RISCV64/ArchSchedule_AI.thy
@@ -14,7 +14,7 @@ named_theorems Schedule_AI_asms
 
 lemma dmo_mapM_storeWord_0_invs[wp,Schedule_AI_asms]:
   "do_machine_op (mapM (\<lambda>p. storeWord p 0) S) \<lbrace>invs\<rbrace>"
-  apply (simp add: dom_mapM ef_storeWord)
+  apply (simp add: dmo_mapM ef_storeWord)
   apply (rule mapM_UNIV_wp)
   apply (simp add: do_machine_op_def split_def)
   apply wp
@@ -25,7 +25,7 @@ lemma dmo_mapM_storeWord_0_invs[wp,Schedule_AI_asms]:
   apply (erule use_valid)
    apply (simp add: storeWord_def word_rsplit_0)
    apply wp
-  apply (simp add: upto.simps)
+  apply (simp add: upto.simps cur_sc_tcb_def)
   done
 
 global_naming Arch
@@ -43,21 +43,16 @@ lemma arch_stt_tcb [wp,Schedule_AI_asms]:
   done
 
 lemma arch_stt_runnable[Schedule_AI_asms]:
-  "\<lbrace>st_tcb_at runnable t\<rbrace> arch_switch_to_thread t \<lbrace>\<lambda>r . st_tcb_at runnable t\<rbrace>"
+  "\<lbrace>st_tcb_at Q t\<rbrace> arch_switch_to_thread t \<lbrace>\<lambda>r . st_tcb_at Q t\<rbrace>"
   apply (simp add: arch_switch_to_thread_def)
   apply wp
   done
-
-lemma idle_strg:
-  "thread = idle_thread s \<and> invs s \<Longrightarrow> invs (s\<lparr>cur_thread := thread\<rparr>)"
-  by (clarsimp simp: invs_def valid_state_def valid_idle_def cur_tcb_def
-                     pred_tcb_at_def valid_machine_state_def obj_at_def is_tcb_def)
 
 lemma arch_stit_invs[wp, Schedule_AI_asms]:
   "\<lbrace>invs\<rbrace> arch_switch_to_idle_thread \<lbrace>\<lambda>r. invs\<rbrace>"
   by (wpsimp simp: arch_switch_to_idle_thread_def)
 
-lemma arch_stit_tcb_at[wp]:
+lemma arch_stit_tcb_at[wp, Schedule_AI_asms]:
   "\<lbrace>tcb_at t\<rbrace> arch_switch_to_idle_thread \<lbrace>\<lambda>r. tcb_at t\<rbrace>"
   apply (simp add: arch_switch_to_idle_thread_def )
   apply (wp tcb_at_typ_at)
@@ -74,12 +69,6 @@ lemma arch_stit_activatable[wp, Schedule_AI_asms]:
   apply (wpsimp simp: ct_in_state_def wp: ct_in_state_thread_state_lift)
   done
 
-lemma stit_invs [wp,Schedule_AI_asms]:
-  "\<lbrace>invs\<rbrace> switch_to_idle_thread \<lbrace>\<lambda>rv. invs\<rbrace>"
-  apply (simp add: switch_to_idle_thread_def arch_switch_to_idle_thread_def)
-  apply (wpsimp|strengthen idle_strg)+
-  done
-
 lemma stit_activatable[Schedule_AI_asms]:
   "\<lbrace>invs\<rbrace> switch_to_idle_thread \<lbrace>\<lambda>rv . ct_in_state activatable\<rbrace>"
   apply (simp add: switch_to_idle_thread_def arch_switch_to_idle_thread_def)
@@ -88,34 +77,22 @@ lemma stit_activatable[Schedule_AI_asms]:
                  elim!: pred_tcb_weaken_strongerE)
   done
 
-lemma stt_invs [wp,Schedule_AI_asms]:
-  "\<lbrace>invs\<rbrace> switch_to_thread t' \<lbrace>\<lambda>_. invs\<rbrace>"
-  apply (simp add: switch_to_thread_def)
-  apply wp
-     apply (simp add: trans_state_update[symmetric] del: trans_state_update)
-    apply (rule_tac Q="\<lambda>_. invs and tcb_at t'" in hoare_strengthen_post, wp)
-    apply (clarsimp simp: invs_def valid_state_def valid_idle_def
-                          valid_irq_node_def valid_machine_state_def)
-    apply (fastforce simp: cur_tcb_def obj_at_def
-                     elim: valid_pspace_eqI ifunsafe_pspaceI)
-   apply wp+
-  apply clarsimp
-  apply (simp add: is_tcb_def)
-  done
-end
+crunch scheduler_action[wp]: set_vm_root "\<lambda>s. P (scheduler_action s)"
 
-interpretation Schedule_AI_U?: Schedule_AI_U
-  proof goal_cases
-  interpret Arch .
-  case 1 show ?case
-  by (intro_locales; (unfold_locales; fact Schedule_AI_asms)?)
-  qed
+lemma arch_stt_scheduler_action [wp, Schedule_AI_asms]:
+  "\<lbrace>\<lambda>s. P (scheduler_action s)\<rbrace> arch_switch_to_thread t' \<lbrace>\<lambda>_ s. P (scheduler_action s)\<rbrace>"
+  by (wpsimp simp: arch_switch_to_thread_def)
+
+lemma arch_stit_scheduler_action [wp, Schedule_AI_asms]:
+  "\<lbrace>\<lambda>s. P (scheduler_action s)\<rbrace> arch_switch_to_idle_thread \<lbrace>\<lambda>_ s. P (scheduler_action s)\<rbrace>"
+  by (wpsimp simp: arch_switch_to_idle_thread_def)
+
+end
 
 interpretation Schedule_AI?: Schedule_AI
   proof goal_cases
   interpret Arch .
-  case 1 show ?case
-  by (intro_locales; (unfold_locales; fact Schedule_AI_asms)?)
+  case 1 show ?case by (intro_locales; (unfold_locales; fact Schedule_AI_asms)?)
   qed
 
 end
